
@prefix :        <http://ns.nature.com/terms/> .
@prefix bibo:    <http://purl.org/ontology/bibo/> .
@prefix dc:      <http://purl.org/dc/elements/1.1/> .
@prefix dcterms: <http://purl.org/dc/terms/> .
@prefix event:   <http://purl.org/NET/c4dm/event.owl#> .
@prefix fabio:   <http://purl.org/spar/fabio/> .
@prefix foaf:    <http://xmlns.com/foaf/0.1/> .
@prefix npg:     <http://ns.nature.com/terms/> .
@prefix npgd:    <http://ns.nature.com/datasets/> .
@prefix npgg:    <http://ns.nature.com/graphs/> .
@prefix skos:    <http://www.w3.org/2004/02/skos/core#> .
@prefix vann:    <http://purl.org/vocab/vann/> .
@prefix owl: <http://www.w3.org/2002/07/owl#> .
@prefix rdf: <http://www.w3.org/1999/02/22-rdf-syntax-ns#> .
@prefix rdfs: <http://www.w3.org/2000/01/rdf-schema#> .
@prefix schema: <http://schema.org/> .
@prefix schemax: <http://topbraid.org/schemax/> .
@prefix xsd: <http://www.w3.org/2001/XMLSchema#> .



@prefix ao: <http://purl.org/ontology/ao/core#> .
@prefix bio: <http://purl.org/vocab/bio/0.1/> .
@prefix cc: <http://web.resource.org/cc/> .
@prefix dc: <http://purl.org/dc/elements/1.1/> .
@prefix dcterms: <http://purl.org/dc/terms/> .
@prefix event: <http://purl.org/NET/c4dm/event.owl#> .
@prefix foaf: <http://xmlns.com/foaf/0.1/> .
@prefix frbr: <http://purl.org/vocab/frbr/core#> .
@prefix geo: <http://www.w3.org/2003/01/geo/wgs84_pos#> .
@prefix keys: <http://purl.org/NET/c4dm/keys.owl#> .
@prefix mo: <http://purl.org/ontology/mo/> .
@prefix owl: <http://www.w3.org/2002/07/owl#> .
@prefix p_file_: <data/schemas/musicontology.rdf> .
@prefix rdf: <http://www.w3.org/1999/02/22-rdf-syntax-ns#> .
@prefix rdfs: <http://www.w3.org/2000/01/rdf-schema#> .
@prefix skos: <http://www.w3.org/2004/02/skos/core#> .
@prefix time: <http://www.w3.org/2006/time#> .
@prefix vs: <http://www.w3.org/2003/06/sw-vocab-status/ns#> .
@prefix wot: <http://xmlns.com/wot/0.1/> .
@prefix xml: <http://www.w3.org/XML/1998/namespace> .
@prefix xsd: <http://www.w3.org/2001/XMLSchema#> .




npg:  a       owl:Ontology ;
      npg:webpage <http://www.nature.com/ontologies/core/> ;
      dc:creator "Tony Hammond <mailto:tony.hammond@macmillan.com>" , "Michele Pasin <mailto:michele.pasin@macmillan.com>" ;
      dc:date "2015-05-21T13:02:15Z" ;
      dc:publisher "Macmillan Publishers Limited" ;
      dc:rights "This work is distributed under a Creative Commons Attribution 4.0 (CC BY 4.0) License <http://creativecommons.org/licenses/by/4.0/>."@en ;
      dcterms:license <http://creativecommons.org/licenses/by/4.0/> ;
      <http://purl.org/vocab/vann/preferredNamespacePrefix>
              "npg" ;
      <http://purl.org/vocab/vann/preferredNamespaceUri>
              "http://ns.nature.com/terms/" ;
      owl:imports <http://www.w3.org/2004/02/skos/core> ;
      owl:versionInfo "1.0.42-SNAPSHOT" ;
      skos:definition "The Core Ontology is a formal model providing definitions for the key concepts of interest to content publishing at Macmillan Science and Education."@en ;
      skos:note "For further information about this ontology or for any queries please use the contact address <mailto:developers@nature.com>."@en ;
      skos:prefLabel "Core Ontology"@en .

npg:Abstract
      a       owl:Class ;
      rdfs:isDefinedBy npg: ;
      rdfs:subClassOf npg:Component ;
      owl:equivalentClass <http://purl.org/spar/fabio/Abstract> ;
      skos:definition "The :Abstract class represents a brief description of a scholarly work, usually author generated. Instances of :Abstract normally do not exist in isolation, but are linked to a :Document instance (of which they provide a summary)."@en ;
      skos:prefLabel "Abstract"@en .

npg:Agent
      a       owl:Class ;
      rdfs:isDefinedBy npg: ;
      rdfs:subClassOf npg:Thing ;
      owl:equivalentClass foaf:Agent ;
      skos:definition "The :Agent class groups together all entities that can be the subject of an action. These can be single persons (:Person), or groups of people organised as a legal entity (:Organization)."@en ;
      skos:prefLabel "Agent"@en .

npg:AggregationEvent
      a       owl:Class ;
      rdfs:isDefinedBy npg: ;
      rdfs:subClassOf npg:Event ;
      skos:definition "The :AggregationEvent class groups together all events related to the construction of a publication."@en ;
      skos:prefLabel "Aggregation Event"@en .

npg:Article
      a       owl:Class ;
      rdfs:isDefinedBy npg: ;
      rdfs:subClassOf npg:Document ;
      owl:equivalentClass <http://purl.org/spar/fabio/Article> , bibo:Article ;
      skos:definition "The :Article class represents a scholarly work normally published as an item of a serial publication. In particular, this concept refers to the abstract notion of an article, rather than any of its realisations after it becomes embodied via a physical medium."@en ;
      skos:note "With reference to the FRBR model [http://www.ifla.org/publications/functional-requirements-for-bibliographic-records], an :Article can be mapped directly to the frbr:Expression concept. It is worth noting though that within the NPG core ontology we do not have any notion of a frbr:Work. Hence multiple versions of the same article (e.g. language translations, or revisions) are characterised as such simply by means of some relationship."@en ;
      skos:prefLabel "Article"@en .

npg:ArticleType
      a       owl:Class ;
      rdfs:isDefinedBy npg: ;
      rdfs:subClassOf npg:Type ;
      skos:definition "The :ArticleType class represents the various kinds of publication which can be used to index and group content published by Macmillan Science and Education. The instances of :ArticleType are organised hierarchically using the SKOS vocabulary."@en ;
      skos:prefLabel "Article Type"@en .

npg:Asset
      a       owl:Class ;
      rdfs:isDefinedBy npg: ;
      rdfs:subClassOf npg:Thing ;
      skos:definition "The :Asset class groups together all physical entities which can be stored in digital systems."@en ;
      skos:prefLabel "Asset"@en .

npg:BinaryAsset
      a       owl:Class ;
      rdfs:isDefinedBy npg: ;
      rdfs:subClassOf npg:BlobAsset ;
      skos:definition "The :BinaryAsset class represents the physical rendition of a generic binary object."@en ;
      skos:prefLabel "Binary Asset"@en .

npg:BlobAsset
      a       owl:Class ;
      rdfs:isDefinedBy npg: ;
      rdfs:subClassOf npg:Asset ;
      skos:definition "The :BlobAsset class groups together all assets used to store blobs - i.e. documents, images, or other media objects - within digital systems."@en ;
      skos:prefLabel "Blob Asset"@en .

npg:Blog
      a       owl:Class ;
      rdfs:isDefinedBy npg: ;
      rdfs:subClassOf npg:Serial ;
      owl:disjointWith npg:Journal ;
      skos:definition "The :Blog class represents an informal serial publication."@en ;
      skos:prefLabel "Blog"@en .

npg:BlogPost
      a       owl:Class ;
      rdfs:isDefinedBy npg: ;
      rdfs:subClassOf npg:Document ;
      skos:definition "The :BlogPost class represents an informal work published as an item of a :Blog."@en ;
      skos:prefLabel "Blog Post"@en .

npg:Collection
      a       owl:Class ;
      rdfs:isDefinedBy npg: ;
      rdfs:subClassOf npg:Document ;
      owl:disjointWith npg:Article ;
      owl:equivalentClass bibo:Collection ;
      skos:definition "The :Collection class represents a group of documents which are published (or republished) as part of a new composite publication. Often these documents have been published elsewhere, but since they share a common theme or belong to an identifiable narrative it is of interest to publish them again within a different container. (See also :Issue.)"@en ;
      skos:prefLabel "Collection"@en .

npg:Component
      a       owl:Class ;
      rdfs:isDefinedBy npg: ;
      rdfs:subClassOf npg:Publication ;
      owl:disjointWith npg:Serial , npg:Document , npg:Dataset ;
      skos:definition "The :Component class groups together all individuals that normally come into existence as part of a :Document."@en ;
      skos:prefLabel "Component"@en .

npg:Concept
      a       owl:Class ;
      rdfs:isDefinedBy npg: ;
      rdfs:subClassOf npg:Thing ;
      owl:equivalentClass skos:Concept ;
      skos:definition "The :Concept class groups together all individuals which do not exist in the physical world (i.e. have no extension in spacetime)."@en ;
      skos:prefLabel "Concept"@en .

npg:Contributor
      a       owl:Class ;
      rdfs:isDefinedBy npg: ;
      rdfs:subClassOf npg:Component ;
      skos:definition "The :Contributor class represents a document component detailing a contributor (personal or corporate) to the work being published. This class is disjoint from the :Agent class. Hence a :Contributor instance can be described as the name used to refer to a person or organisation in the context of a publication."@en ;
      skos:prefLabel "Contributor"@en .

npg:Dataset
      a       owl:Class ;
      rdfs:isDefinedBy npg: ;
      rdfs:subClassOf npg:Publication ;
      skos:definition "The :Dataset class represents a collection of related sets of information modelled in a known way and stored in a computer system."@en ;
      skos:note "We are currently using this class for RDF datasets."@en ;
      skos:prefLabel "Dataset"@en .

npg:Document
      a       owl:Class ;
      rdfs:isDefinedBy npg: ;
      rdfs:subClassOf npg:Publication ;
      owl:disjointWith npg:Serial , npg:Component ;
      skos:definition "The :Document class groups together all publications which were created to be distributed and consumed as individual, self-contained entities."@en ;
      skos:prefLabel "Document"@en .

npg:Event
      a       owl:Class ;
      rdfs:isDefinedBy npg: ;
      rdfs:subClassOf npg:Thing ;
      owl:equivalentClass <http://purl.org/NET/c4dm/event.owl#Event> ;
      skos:definition "The :Event class groups together events of varying granularity. Events differ from :Concept entities because they have an extension in time; they differ from :Asset entities because they do not have an extension in space."@en ;
      skos:prefLabel "Event"@en .

npg:ExternalArticle
      a       owl:Class ;
      rdfs:isDefinedBy npg: ;
      rdfs:subClassOf npg:Article ;
      skos:definition "The :ExternalArticle class represents an article which is externally published."@en ;
      skos:note "The :ExternalArticle class subclasses the :Article class."@en ;
      skos:prefLabel "External Article"@en .

npg:ExternalContributor
      a       owl:Class ;
      rdfs:isDefinedBy npg: ;
      rdfs:subClassOf npg:Contributor ;
      skos:definition "The :ExternalContributor class represents a contributor from an article which is externally published."@en ;
      skos:note "The :ExternalContributor class subclasses the :Contributor class."@en ;
      skos:prefLabel "External Contributor"@en .

npg:Figure
      a       owl:Class ;
      rdfs:isDefinedBy npg: ;
      rdfs:subClassOf npg:Image ;
      owl:disjointWith npg:Illustration ;
      skos:definition "The :Figure class represents a numbered and captioned image within a publication. This image typically results as a direct outcome of the work described in the publication."@en ;
      skos:prefLabel "Figure"@en .

npg:Graph
      a       owl:Class ;
      rdfs:isDefinedBy npg: ;
      rdfs:subClassOf npg:Dataset ;
      owl:disjointWith npg:KnowledgeBase ;
      skos:definition "The :Graph class represents a collection of related sets of information modelled in RDF and organized as a named graph."@en ;
      skos:note "Each Graph instance is associated with instances of a particular class. For example, the 'npgg:articles' :Graph instance is a named graph which contains all the instances of the :Article class. The :Graph instances themselves are then used to describe the RDF graph, providing sometimes known as an RDF annotation. This may furnish various kinds of information about the RDF graph: provenance, rights, metrics, validation reports, etc."@en ;
      skos:prefLabel "Graph"@en .

npg:Illustration
      a       owl:Class ;
      rdfs:isDefinedBy npg: ;
      rdfs:subClassOf npg:Image ;
      owl:disjointWith npg:Figure ;
      skos:definition "The :Illustration class represents a numbered and captioned image within a publication. This image typically illustrates a point about the work described in the publication."@en ;
      skos:prefLabel "Illustration"@en .

npg:Image
      a       owl:Class ;
      rdfs:isDefinedBy npg: ;
      rdfs:subClassOf npg:Component ;
      skos:definition "The :Image class represents a graphical element within a publication."@en ;
      skos:prefLabel "Image"@en .

npg:ImageAsset
      a       owl:Class ;
      rdfs:isDefinedBy npg: ;
      rdfs:subClassOf npg:BlobAsset ;
      skos:definition "The :ImageAsset class represents the physical rendition of an image asset in an encoded format."@en ;
      skos:prefLabel "Image Asset"@en .

npg:Issue
      a       owl:Class ;
      rdfs:isDefinedBy npg: ;
      rdfs:subClassOf npg:Collection ;
      owl:equivalentClass <http://purl.org/spar/fabio/JournalIssue> ;
      skos:definition "The :Issue class represents an aggregate object which is published periodically as part of a :Serial and is normally composed by one or more articles. (See also :Collection.)"@en ;
      skos:prefLabel "Issue"@en .

npg:Item
      a       owl:Class ;
      rdfs:isDefinedBy npg: ;
      rdfs:subClassOf npg:AggregationEvent ;
      skos:definition "The :Item class represents the state of a document after this has been added to a :Collection by someone, at a specific time, and within a specific sequence."@en ;
      skos:prefLabel "Item"@en .

npg:Journal
      a       owl:Class ;
      rdfs:isDefinedBy npg: ;
      rdfs:subClassOf npg:Serial ;
      owl:disjointWith npg:Blog ;
      owl:equivalentClass <http://purl.org/spar/fabio/Journal> ;
      skos:definition "The :Journal class represents a scholarly serial publication, considered from both the scholarly and the commercial perspectives. Thus a journal is more than the sum of its publications (i.e. the set of all the :Issue instances it has published); it is an entity characterised by many properties, e.g. its founders, its impact factor, etc."@en ;
      skos:prefLabel "Journal"@en .

npg:KnowledgeBase
      a       owl:Class ;
      rdfs:isDefinedBy npg: ;
      rdfs:subClassOf npg:Dataset ;
      owl:disjointWith npg:Graph ;
      skos:definition "The :KnowledgeBase class represents a collection of related sets of information modelled in RDF and consisting of various objects, e.g. one or more graphs, other RDF datasets etc."@en ;
      skos:note "Differently from datasets, knowledge-bases refer to a composite dataset intended to be used as a consistent whole."@en ;
      skos:prefLabel "KnowledgeBase"@en .

npg:Organization
      a       owl:Class ;
      rdfs:isDefinedBy npg: ;
      rdfs:subClassOf npg:Agent ;
      owl:equivalentClass foaf:Organization ;
      skos:definition "The :Organization class represents an organised body of people normally having a legal status."@en ;
      skos:prefLabel "Organization"@en .

npg:PdfAsset
      a       owl:Class ;
      rdfs:isDefinedBy npg: ;
      rdfs:subClassOf npg:BlobAsset ;
      skos:definition "The :PdfAsset class represents the physical rendition of a document asset in PDF format."@en ;
      skos:prefLabel "Pdf Asset"@en .

npg:Person
      a       owl:Class ;
      rdfs:isDefinedBy npg: ;
      rdfs:subClassOf npg:Agent ;
      skos:definition "The :Person class represents a single person entity."@en ;
      skos:prefLabel "Person"@en .

npg:Publication
      a       owl:Class ;
      rdfs:isDefinedBy npg: ;
      rdfs:subClassOf npg:Concept ;
      skos:definition "The :Publication class groups together all individuals (or part of) created as the result of the publishing process. Note that we are not referring here to the physical artefacts, but just their abstract counterparts."@en ;
      skos:prefLabel "Publication"@en .

npg:PublicationEvent
      a       owl:Class ;
      rdfs:isDefinedBy npg: ;
      rdfs:subClassOf npg:Event ;
      skos:definition "The :PublicationEvent class groups together events that happen within the publishing process, broadly conceived. For example, the submission of an article, or the acceptance of a paper."@en ;
      skos:prefLabel "Publication Event"@en .

npg:PublicationState
      a       owl:Class ;
      rdfs:isDefinedBy npg: ;
      rdfs:subClassOf npg:Type ;
      skos:definition "The :PublicationState class groups together publish-state and review-state individuals."@en ;
      skos:prefLabel "Publication State"@en .

npg:PublishEvent
      a       owl:Class ;
      rdfs:isDefinedBy npg: ;
      rdfs:subClassOf npg:PublicationEvent ;
      skos:definition "The :PublishEvent class represents events related to the publication of a document. This is intended in a strict sense, i.e. the time when a publication is made 'public'."@en ;
      skos:note "In order to differentiate these events further, the :PublishState vocabulary is used."@en ;
      skos:prefLabel "Publish Event"@en .

npg:PublishState
      a       owl:Class ;
      rdfs:isDefinedBy npg: ;
      rdfs:subClassOf npg:PublicationState ;
      skos:definition "The :PublishState class provides a categorisation of the possible states a document may have after it has been published. For example, whether it’s an 'Advanced online publication' or an 'Issue publication'.  This categorisation is implemented as a SKOS vocabulary."@en ;
      skos:prefLabel "Publish State"@en .

npg:Publisher
      a       owl:Class ;
      rdfs:isDefinedBy npg: ;
      rdfs:subClassOf npg:Organization ;
      skos:definition "The :Publisher class represents organizations involved in the publishing business."@en ;
      skos:prefLabel "Publisher"@en .

npg:ReviewEvent
      a       owl:Class ;
      rdfs:isDefinedBy npg: ;
      rdfs:subClassOf npg:PublicationEvent ;
      skos:definition "The :ReviewEvent class models events related to the reviewing of a document (before its publication). In order to differentiate these events further, the :ReviewState vocabulary is used."@en ;
      skos:prefLabel "Review Event"@en .

npg:ReviewState
      a       owl:Class ;
      rdfs:isDefinedBy npg: ;
      rdfs:subClassOf npg:PublicationState ;
      skos:definition "The :ReviewState class provides a categorisation of the possible states a document may have as a result of a reviewing process. For example, whether it’s been 'Received' or 'Accepted'.  This categorisation is implemented as a SKOS vocabulary."@en ;
      skos:prefLabel "Review State"@en .

npg:Section
      a       owl:Class ;
      rdfs:isDefinedBy npg: ;
      rdfs:subClassOf npg:Component ;
      skos:definition "The :Section class represents a part of a document."@en ;
      skos:prefLabel "Section"@en .

npg:Serial
      a       owl:Class ;
      rdfs:isDefinedBy npg: ;
      rdfs:subClassOf npg:Publication ;
      owl:disjointWith npg:Document , npg:Component , npg:Dataset ;
      owl:equivalentClass <http://purl.org/spar/fabio/Periodical> ;
      skos:definition "The :Serial class represents publications which appear in a new edition on a regular schedule. For example, a journal, a magazine or a blog. The :PublishEvent class is used to provide more details about the time, place and other contextual information relevant to when a new edition gets published."@en ;
      skos:prefLabel "Serial"@en .

npg:SeverityLevel
      a       owl:Class ;
      rdfs:isDefinedBy npg: ;
      rdfs:subClassOf npg:Type ;
      skos:definition "The :SeverityLevel class represents a system status. The syslog standard (RFC 5424) for computer message logging is used to provide a reference set of states. This categorisation is implemented as a SKOS concept scheme."@en ;
      skos:prefLabel "Severity Level"@en .

npg:Subject
      a       owl:Class ;
      rdfs:isDefinedBy npg: ;
      rdfs:subClassOf npg:Type ;
      owl:equivalentClass <http://purl.org/spar/fabio/SubjectTerm> ;
      skos:definition "The :Subject class represents a topic, field of study or research area which can be used to categorise the contents of a publication. The instances of :Subject are organised hierarchically using the SKOS vocabulary."@en ;
      skos:prefLabel "Subject"@en .

npg:Summary
      a       owl:Class ;
      rdfs:isDefinedBy npg: ;
      rdfs:subClassOf npg:Component ;
      skos:definition "The :Summary class represents a brief description of a scholarly work, usually editorially generated."@en ;
      skos:prefLabel "Summary"@en .

npg:SummaryType
      a       owl:Class ;
      rdfs:isDefinedBy npg: ;
      rdfs:subClassOf npg:Type ;
      skos:definition "The :SummaryType class represents an instance from  a categorisation of types of :Summary. For example, 'Long Summary', 'Short Summary', etc. This categorisation is implemented as a SKOS concept scheme."@en ;
      skos:prefLabel "Summary Type"@en .

npg:Thing
      a       owl:Class ;
      rdfs:isDefinedBy npg: ;
      rdfs:subClassOf owl:Thing ;
      skos:definition "The :Thing class groups together all individuals used by Macmillan Science and Education within the NPG publishing world."@en ;
      skos:prefLabel "Thing"@en .

npg:Type
      a       owl:Class ;
      rdfs:isDefinedBy npg: ;
      rdfs:subClassOf npg:Concept ;
      skos:definition "The :Type class groups together  all domain-specific categorisations relevant to the NPG publishing world."@en ;
      skos:note "All of the :Type categorisations are implemented as self-contained reusable SKOS vocabularies (although not all of them are taxonomies in the strict sense of hierarchical vocabularies)."@en ;
      skos:prefLabel "Type"@en .

npg:Website
      a       owl:Class ;
      rdfs:isDefinedBy npg: ;
      rdfs:subClassOf npg:Publication ;
      skos:definition "The :Website class represents a site that maintains one or more pages on the Web."@en ;
      skos:prefLabel "Website"@en .

npg:XmlAsset
      a       owl:Class ;
      rdfs:isDefinedBy npg: ;
      rdfs:subClassOf npg:Asset ;
      skos:definition "The :XmlAsset class represents the physical rendition of a document asset in XML format."@en ;
      skos:prefLabel "Xml Asset"@en .

npg:assetFolderName
      a       owl:DatatypeProperty ;
      rdfs:domain npg:Journal ;
      rdfs:isDefinedBy npg: ;
      rdfs:range rdfs:Literal ;
      skos:definition "The :assetFolderName property specifies a folder name for file storage assets."@en ;
      skos:prefLabel "Asset Folder Name"@en .

npg:assetVersion
      a       owl:DatatypeProperty ;
      rdfs:domain npg:Asset ;
      rdfs:isDefinedBy npg: ;
      rdfs:range rdfs:Literal ;
      skos:definition "The :assetVersion property specifies the version of an :Asset associated with a :PublishEvent."@en ;
      skos:prefLabel "Asset Version"@en .

npg:baseUriTemplate
      a       owl:DatatypeProperty ;
      rdfs:isDefinedBy npg: ;
      rdfs:range rdfs:Literal ;
      skos:definition "The :baseUriTemplate property specifies a string template for an asset base URI."@en ;
      skos:prefLabel "Base URI Template"@en .

npg:body
      a       owl:DatatypeProperty ;
      rdfs:domain npg:Publication ;
      rdfs:isDefinedBy npg: ;
      rdfs:range rdfs:Literal ;
      skos:definition "The :body property specifies the main body content of a publication as a string."@en ;
      skos:prefLabel "Body"@en .

npg:bodyXml
      a       owl:DatatypeProperty ;
      rdfs:domain npg:Publication ;
      rdfs:isDefinedBy npg: ;
      rdfs:range rdfs:Literal ;
      skos:definition "The :bodyXml property specifies the main body content of a publication as an XML string."@en ;
      skos:prefLabel "Body (XML)"@en .

npg:caption
      a       owl:DatatypeProperty ;
      rdfs:domain npg:Image ;
      rdfs:isDefinedBy npg: ;
      rdfs:range rdfs:Literal ;
      skos:definition "The :caption property specifies the caption of a figure or illustration as a string."@en ;
      skos:prefLabel "Caption"@en .

npg:captionXml
      a       owl:DatatypeProperty ;
      rdfs:domain npg:Image ;
      rdfs:isDefinedBy npg: ;
      rdfs:range rdfs:Literal ;
      skos:definition "The :captionXml property specifies the caption of a figure or illustration as an XML string."@en ;
      skos:prefLabel "Caption (XML)"@en .

npg:citation
      a       owl:DatatypeProperty ;
      rdfs:domain npg:Publication ;
      rdfs:isDefinedBy npg: ;
      rdfs:range rdfs:Literal ;
      skos:definition "The :citation property specifies the full citation of a publication as a single string for reference purposes."@en ;
      skos:prefLabel "Citation"@en .

npg:citationData
      a       owl:DatatypeProperty ;
      rdfs:domain npg:Publication ;
      rdfs:isDefinedBy npg: ;
      rdfs:range rdfs:Literal ;
      skos:definition "The :citationData property specifies the full citation of a publication as a single string for machine use."@en ;
      skos:note "This is an alternative representation of the :citation property."@en ;
      skos:prefLabel "Citation (Data)"@en .

npg:citationXml
      a       owl:DatatypeProperty ;
      rdfs:domain npg:Publication ;
      rdfs:isDefinedBy npg: ;
      rdfs:range rdfs:Literal ;
      skos:definition "The :citationXML property specifies the full citation of a publication as a single string containing XML for user presentation."@en ;
      skos:note "This is an alternative representation of the :citation property."@en ;
      skos:prefLabel "Citation (XML)"@en .

npg:class
      a       owl:AnnotationProperty ;
      rdfs:isDefinedBy npg: ;
      skos:definition "The :class property specifies the class a domain model refers to."@en ;
      skos:prefLabel "Class"@en .

npg:code
      a       owl:DatatypeProperty ;
      rdfs:domain npg:Type ;
      rdfs:isDefinedBy npg: ;
      rdfs:range xsd:integer ;
      skos:definition "The :code property specifies an integer number representing an internal ID for an object."@en ;
      skos:note "This property is used by the doamin ontologies for managing terms."@en ;
      skos:prefLabel "Code"@en .

npg:contributorList
      a       owl:ObjectProperty ;
      rdfs:domain npg:Publication ;
      rdfs:isDefinedBy npg: ;
      rdfs:range rdf:List ;
      owl:equivalentProperty
              bibo:contributorList ;
      skos:definition "The :contributorList property specifies an ordered list of contributors."@en ;
      skos:prefLabel "Contributor List"@en .

npg:count
      a       owl:ObjectProperty ;
      rdfs:isDefinedBy npg: ;
      skos:definition "The :count property specifies a map which records the number of instances of an entity."@en ;
      skos:prefLabel "Count"@en .

npg:coverDate
      a       owl:DatatypeProperty ;
      rdfs:domain npg:Publication ;
      rdfs:isDefinedBy npg: ;
      rdfs:range xsd:date ;
      skos:definition "The :coverDate property specifies the full date of a publication as it is displayed on its cover."@en ;
      skos:note "This is not necessarily the actual date of publication."@en ;
      skos:prefLabel "Cover Date"@en .

npg:coverYear
      a       owl:DatatypeProperty ;
      rdfs:domain npg:Publication ;
      rdfs:isDefinedBy npg: ;
      rdfs:range xsd:gYear ;
      skos:definition "The :coverDate property specifies the year date of a publication as it is displayed on its cover."@en ;
      skos:note "This is not necessarily the actual date of publication."@en ;
      skos:prefLabel "Cover Year"@en .

npg:coverYearMonth
      a       owl:DatatypeProperty ;
      rdfs:domain npg:Publication ;
      rdfs:isDefinedBy npg: ;
      rdfs:range xsd:gYearMonth ;
      skos:definition "The :coverDate property specifies the year and month date of a publication as it is displayed on its cover."@en ;
      skos:note "This is not necessarily the actual date of publication."@en ;
      skos:prefLabel "Cover YearMonth"@en .

npg:credit
      a       owl:DatatypeProperty ;
      rdfs:domain npg:Image ;
      rdfs:isDefinedBy npg: ;
      rdfs:range rdfs:Literal ;
      skos:definition "The :credit property specifies the photographer, illustrator, or copyright holder for an image in a publication."@en ;
      skos:prefLabel "Credit"@en .

npg:date
      a       owl:DatatypeProperty ;
      rdfs:domain npg:Event ;
      rdfs:isDefinedBy npg: ;
      rdfs:range xsd:date ;
      skos:definition "The :date property specifies the full date of an event as a string."@en ;
      skos:prefLabel "Date"@en .

npg:dateEnd
      a       owl:DatatypeProperty ;
      rdfs:domain npg:Serial ;
      rdfs:isDefinedBy npg: ;
      rdfs:range rdfs:Literal ;
      skos:definition "The :dateEnd property specifies the end date for a serial publication."@en ;
      skos:prefLabel "Date End"@en .

npg:dateStart
      a       owl:DatatypeProperty ;
      rdfs:domain npg:Serial ;
      rdfs:isDefinedBy npg: ;
      rdfs:range rdfs:Literal ;
      skos:definition "The :dateStart property specifies the start date for a serial publication."@en ;
      skos:prefLabel "Date Start"@en .

npg:dateTime
      a       owl:DatatypeProperty ;
      rdfs:domain npg:Event ;
      rdfs:isDefinedBy npg: ;
      rdfs:range xsd:dateTime ;
      skos:definition "The :dateTime property specifies the full date of an event as a string, including a time component."@en ;
      skos:prefLabel "DateTime"@en .

npg:datetime
      a       owl:AnnotationProperty ;
      rdfs:isDefinedBy npg: ;
      skos:definition "The :datetime property specifies a system-generated datetime for an entity."@en ;
      skos:prefLabel "Datetime"@en .

npg:doi
      a       owl:DatatypeProperty ;
      rdfs:domain npg:Publication ;
      rdfs:isDefinedBy npg: ;
      rdfs:range rdfs:Literal ;
      owl:equivalentProperty
              bibo:doi ;
      skos:definition "The :doi property specifies a DOI number for a publication."@en ;
      skos:prefLabel "DOI"@en .

npg:doiLink
      a       owl:ObjectProperty ;
      rdfs:domain npg:Publication ;
      rdfs:isDefinedBy npg: ;
      skos:definition "The :doiLink property relates a publication to the URI minted from the DOI."@en ;
      skos:prefLabel "DOI Link"@en .

npg:eissn
      a       owl:DatatypeProperty ;
      rdfs:domain npg:Serial ;
      rdfs:isDefinedBy npg: ;
      rdfs:range rdfs:Literal ;
      owl:equivalentProperty
              bibo:eissn ;
      skos:definition "The :eissn property specifies an E-ISSN number for a serial."@en ;
      skos:prefLabel "E-ISSN"@en .

npg:example
      a       owl:AnnotationProperty ;
      rdfs:isDefinedBy npg: ;
      skos:definition "The :example property specifies an example of an entity."@en ;
      skos:note "This property is similar to void:exampleResource. But see also skos:example."@en ;
      skos:prefLabel "Example"@en .

npg:familyName
      a       owl:DatatypeProperty ;
      rdfs:domain npg:Contributor ;
      rdfs:isDefinedBy npg: ;
      rdfs:range rdfs:Literal ;
      owl:equivalentProperty
              foaf:familyName ;
      skos:definition "The :familyName property specifies the family name of a person."@en ;
      skos:prefLabel "Family Name"@en .

npg:figureList
      a       owl:ObjectProperty ;
      rdfs:domain npg:Publication ;
      rdfs:isDefinedBy npg: ;
      rdfs:range rdf:List ;
      skos:definition "The :figureList property specifies an ordered list of figures for a publication."@en ;
      skos:prefLabel "Figure List"@en .

npg:fileExtension
      a       owl:DatatypeProperty ;
      rdfs:domain npg:Asset ;
      rdfs:isDefinedBy npg: ;
      rdfs:range rdfs:Literal ;
      skos:definition "The :fileExtension property specifies the extension part of the filename of an asset."@en ;
      skos:prefLabel "File Extension"@en .

npg:filename
      a       owl:DatatypeProperty ;
      rdfs:domain npg:Asset ;
      rdfs:isDefinedBy npg: ;
      rdfs:range rdfs:Literal ;
      skos:definition "The :filename property specifies the filename of an asset."@en ;
      skos:prefLabel "Filename"@en .

npg:filesize
      a       owl:DatatypeProperty ;
      rdfs:domain npg:Asset ;
      rdfs:isDefinedBy npg: ;
      rdfs:range rdfs:Literal ;
      skos:definition "The :filesize property specifies an integer value for the size (in bytes) of an asset."@en ;
      skos:prefLabel "Filesize"@en .

npg:givenName
      a       owl:DatatypeProperty ;
      rdfs:domain npg:Contributor ;
      rdfs:isDefinedBy npg: ;
      rdfs:range rdfs:Literal ;
      owl:equivalentProperty
              foaf:givenName ;
      skos:definition "The :givenName property specifies the given name of a person."@en ;
      skos:prefLabel "Given Name"@en .

npg:graph
      a       owl:AnnotationProperty ;
      rdfs:isDefinedBy npg: ;
      skos:definition "The :graph property specifies the full URI of any graph."@en ;
      skos:prefLabel "Graph"@en .

npg:hasAbstract
      a       owl:ObjectProperty ;
      rdfs:domain npg:Article ;
      rdfs:isDefinedBy npg: ;
      rdfs:range npg:Abstract ;
      skos:definition "The :hasAbstract property relates an article to the abstract for an article."@en ;
      skos:prefLabel "Has Abstract"@en .

npg:hasArticle
      a       owl:ObjectProperty ;
      rdfs:domain npg:PublicationEvent ;
      rdfs:isDefinedBy npg: ;
      rdfs:range npg:Article ;
      skos:definition "The :hasArticle property relates a publication-event to an article."@en ;
      skos:prefLabel "Has Article"@en .

npg:hasArticleType
      a       owl:ObjectProperty ;
      rdfs:domain npg:Article ;
      rdfs:isDefinedBy npg: ;
      rdfs:range npg:ArticleType ;
      skos:definition "The :hasArticleType relates an article to an article-type."@en ;
      skos:prefLabel "Has Article Type"@en .

npg:hasAsset
      a       owl:ObjectProperty ;
      rdfs:domain npg:Publication ;
      rdfs:isDefinedBy npg: ;
      rdfs:range npg:Asset ;
      skos:definition "The :hasAsset property relates a publication to an asset."@en ;
      skos:prefLabel "Has Asset"@en .

npg:hasBlog
      a       owl:ObjectProperty ;
      rdfs:isDefinedBy npg: ;
      rdfs:range npg:Blog ;
      rdfs:subPropertyOf npg:hasSerial ;
      skos:definition "The :hasBlog property relates a serial to a blog associated with it."@en ;
      skos:prefLabel "Has Blog"@en .

npg:hasBroaderSubject
      a       owl:ObjectProperty ;
      rdfs:domain npg:Publication ;
      rdfs:isDefinedBy npg: ;
      rdfs:range npg:Subject ;
      rdfs:subPropertyOf npg:hasSubject ;
      skos:definition "The :hasBroaderSubject property relates a publication to a broader subject term than it is actually classified with."@en ;
      skos:prefLabel "Has Broader Subject"@en .

npg:hasCollection
      a       owl:ObjectProperty ;
      rdfs:domain npg:PublicationEvent ;
      rdfs:isDefinedBy npg: ;
      rdfs:range npg:Collection ;
      skos:definition "The :hasCollection property relates a publication-event to a collection."@en ;
      skos:prefLabel "Has Collection"@en .

npg:hasContributor
      a       owl:ObjectProperty ;
      rdfs:domain npg:Document ;
      rdfs:isDefinedBy npg: ;
      rdfs:range npg:Contributor ;
      skos:definition "The :hasContributor property relates a publication to a string containing the name of one of the authors of that publication."@en ;
      skos:note "Normally, the contributor name is a non-disambiguated person name, meaning that several contributor instances may refer to the same person."@en ;
      skos:prefLabel "Has Contributor"@en .

npg:hasCorrespondingContributor
      a       owl:ObjectProperty ;
      rdfs:domain npg:Article ;
      rdfs:isDefinedBy npg: ;
      rdfs:range npg:Contributor ;
      rdfs:subPropertyOf npg:hasContributor ;
      skos:definition "The :hasCorrespondingContributor property relates an article to the name of its corresponding author."@en ;
      skos:prefLabel "Has Corresponding Contributor"@en .

npg:hasCurrentIssue
      a       owl:ObjectProperty ;
      rdfs:domain npg:Publication ;
      rdfs:isDefinedBy npg: ;
      rdfs:range npg:Issue ;
      rdfs:subPropertyOf npg:hasIssue ;
      skos:definition "The :hasCurrentIssue property relates a publication to the current issue."@en ;
      skos:prefLabel "Has Current Issue"@en .

npg:hasExternalArticle
      a       owl:ObjectProperty ;
      rdfs:domain npg:Article ;
      rdfs:isDefinedBy npg: ;
      rdfs:range npg:ExternalArticle ;
      skos:definition "The :hasExternalArticle property relates an article to an external article."@en ;
      skos:prefLabel "Has External Article"@en .

npg:hasExternalContributor
      a       owl:ObjectProperty ;
      rdfs:domain npg:Article ;
      rdfs:isDefinedBy npg: ;
      rdfs:range npg:ExternalContributor ;
      skos:definition "The :hasExternalArticle property relates an article to an external contributor."@en ;
      skos:prefLabel "Has External Contributor"@en .

npg:hasFigure
      a       owl:ObjectProperty ;
      rdfs:domain npg:Publication ;
      rdfs:isDefinedBy npg: ;
      rdfs:range npg:Figure ;
      skos:definition "The :hasFigure property relates a publication to a figure."@en ;
      skos:prefLabel "Has Figure"@en .

npg:hasGraph
      a       owl:ObjectProperty ;
      rdfs:isDefinedBy npg: ;
      rdfs:range npg:Graph ;
      skos:definition "The :hasGraph property relates an entity to the RDF named graph associated with it."@en ;
      skos:prefLabel "Has Graph"@en .

npg:hasIllustration
      a       owl:ObjectProperty ;
      rdfs:domain npg:Publication ;
      rdfs:isDefinedBy npg: ;
      rdfs:range npg:Illustration ;
      skos:definition "The :hasIllustration property relates a publication to an illustration."@en ;
      skos:prefLabel "Has Illustration"@en .

npg:hasImage
      a       owl:ObjectProperty ;
      rdfs:domain npg:Publication ;
      rdfs:isDefinedBy npg: ;
      rdfs:range npg:Image ;
      skos:definition "The :hasImage property relates a publication to an image."@en ;
      skos:prefLabel "Has Image"@en .

npg:hasImageAsset
      a       owl:ObjectProperty ;
      rdfs:domain npg:Image ;
      rdfs:isDefinedBy npg: ;
      rdfs:range npg:ImageAsset ;
      skos:definition "The :hasImageAsset property relates an image to an image-asset."@en ;
      skos:prefLabel "Has Image Asset"@en .

npg:hasIssue
      a       owl:ObjectProperty ;
      rdfs:domain npg:PublicationEvent ;
      rdfs:isDefinedBy npg: ;
      rdfs:range npg:Issue ;
      skos:definition "The :hasIssue property relates a publication-event to an issue."@en ;
      skos:prefLabel "Has Issue"@en .

npg:hasItem
      a       owl:ObjectProperty ;
      rdfs:domain npg:Publication ;
      rdfs:isDefinedBy npg: ;
      rdfs:range npg:Item ;
      skos:definition "The :hasItem property relates a publication to an item."@en ;
      skos:prefLabel "Has Item"@en .

npg:hasJournal
      a       owl:ObjectProperty ;
      rdfs:isDefinedBy npg: ;
      rdfs:range npg:Journal ;
      rdfs:subPropertyOf npg:hasSerial ;
      skos:definition "The :hasJournal property relates a publication to a journal."@en ;
      skos:prefLabel "Has Journal"@en .

npg:hasNextIssue
      a       owl:ObjectProperty ;
      rdfs:domain npg:Publication ;
      rdfs:isDefinedBy npg: ;
      rdfs:range npg:Issue ;
      rdfs:subPropertyOf npg:hasIssue ;
      skos:definition "The :hasNextIssue property relates a publication to the next issue."@en ;
      skos:prefLabel "Has Next Issue"@en .

npg:hasPdfAsset
      a       owl:ObjectProperty ;
      rdfs:domain npg:Publication ;
      rdfs:isDefinedBy npg: ;
      rdfs:range npg:PdfAsset ;
      skos:definition "The :hasPdfAsset property relates a publication to a pdf-asset."@en ;
      skos:prefLabel "Has PDF Asset"@en .

npg:hasPreviousIssue
      a       owl:ObjectProperty ;
      rdfs:domain npg:Publication ;
      rdfs:isDefinedBy npg: ;
      rdfs:range npg:Issue ;
      rdfs:subPropertyOf npg:hasIssue ;
      skos:definition "The :hasPreviousIssue property relates a publication to the previous issue."@en ;
      skos:prefLabel "Has Previous Issue"@en .

npg:hasPrimaryArticleType
      a       owl:ObjectProperty ;
      rdfs:domain npg:Article ;
      rdfs:isDefinedBy npg: ;
      rdfs:range npg:ArticleType ;
      rdfs:subPropertyOf npg:hasArticleType ;
      skos:definition "The :hasPrimaryArticleType property relates an article to an article-type that can be used for grouping purposes."@en ;
      skos:prefLabel "Has Primary Article Type"@en .

npg:hasPublication
      a       owl:ObjectProperty ;
      rdfs:domain npg:PublicationEvent ;
      rdfs:isDefinedBy npg: ;
      rdfs:range npg:Publication ;
      skos:definition "The :hasPublication property relates a publication-event to a publication."@en ;
      skos:prefLabel "Has Publication"@en .

npg:hasPublishEvent
      a       owl:ObjectProperty ;
      rdfs:domain npg:Publication ;
      rdfs:isDefinedBy npg: ;
      rdfs:range npg:PublishEvent ;
      skos:definition "The :hasPublishEvent property relates a publication to a publish-event that describes some recognized change in the status of a publication's publish history."@en ;
      skos:prefLabel "Has Publish Event"@en .

npg:hasPublishState
      a       owl:ObjectProperty ;
      rdfs:domain npg:PublishEvent ;
      rdfs:isDefinedBy npg: ;
      rdfs:range npg:PublishState ;
      skos:definition "The :hasPublishState property relates a publish-event to a publish-state that describes some recognized change in the status of a publication's publish history."@en ;
      skos:prefLabel "Has Publish State"@en .

npg:hasPublisher
      a       owl:ObjectProperty ;
      rdfs:domain npg:Publication ;
      rdfs:isDefinedBy npg: ;
      rdfs:range npg:Publisher ;
      owl:equivalentProperty
              dcterms:publisher ;
      skos:definition "The :hasPublisher property relates a publication to the organization that publishes it."@en ;
      skos:prefLabel "Has Publisher"@en .

npg:hasReviewEvent
      a       owl:ObjectProperty ;
      rdfs:domain npg:Publication ;
      rdfs:isDefinedBy npg: ;
      rdfs:range npg:ReviewEvent ;
      skos:definition "The :hasReviewEvent property relates a publication to a review-event that describes some recognized change in the status of a publication's review history."@en ;
      skos:prefLabel "Has Review Event"@en .

npg:hasReviewState
      a       owl:ObjectProperty ;
      rdfs:domain npg:ReviewEvent ;
      rdfs:isDefinedBy npg: ;
      rdfs:range npg:ReviewState ;
      skos:definition "The :hasReviewState property relates a review-event to a review-state that describes some recognized change in the status of a publication's review history."@en ;
      skos:prefLabel "Has Review State"@en .

npg:hasRoot
      a       owl:ObjectProperty ;
      rdfs:domain npg:Type ;
      rdfs:isDefinedBy npg: ;
      rdfs:range npg:Type ;
      skos:definition "The :hasRoot property relates a :Type instance to a toplevel :Type instance within the same domain model."@en ;
      skos:prefLabel "Has Root"@en .

npg:hasSection
      a       owl:ObjectProperty ;
      rdfs:domain npg:Item ;
      rdfs:isDefinedBy npg: ;
      rdfs:range npg:Section ;
      skos:definition "The :hasSection property relates an item to a section component."@en ;
      skos:prefLabel "Has Section"@en .

npg:hasSerial
      a       owl:ObjectProperty ;
      rdfs:domain npg:Publication ;
      rdfs:isDefinedBy npg: ;
      rdfs:range npg:Serial ;
      skos:definition "The :hasSerial property relates a publication to a serial."@en ;
      skos:prefLabel "Has Serial"@en .

npg:hasSubject
      a       owl:ObjectProperty ;
      rdfs:domain npg:Publication ;
      rdfs:isDefinedBy npg: ;
      rdfs:range npg:Subject ;
      owl:equivalentProperty
              <http://purl.org/spar/fabio/hasSubjectTerm> ;
      skos:definition "The :hasSubject property relates a publication to a subject term which describes one of the main topics the publication is about."@en ;
      skos:prefLabel "Has Subject"@en .

npg:hasSummary
      a       owl:ObjectProperty ;
      rdfs:domain npg:Article ;
      rdfs:isDefinedBy npg: ;
      rdfs:range npg:Summary ;
      skos:definition "The :hasSummary property relates an article to an article summary."@en ;
      skos:prefLabel "Has Summary"@en .

npg:hasSummaryType
      a       owl:ObjectProperty ;
      rdfs:domain npg:Summary ;
      rdfs:isDefinedBy npg: ;
      rdfs:range npg:SummaryType ;
      skos:definition "The :hasSummaryType property relates a summary to a summary-type classification."@en ;
      skos:prefLabel "Has Summary Type"@en .

npg:hasWebsite
      a       owl:ObjectProperty ;
      rdfs:domain npg:Publication ;
      rdfs:isDefinedBy npg: ;
      rdfs:range npg:Website ;
      rdfs:subPropertyOf npg:hasSerialPublication ;
      skos:definition "The :hasWebsite property relates a publication to a website."@en ;
      skos:prefLabel "Has Website"@en .

npg:hasXmlAsset
      a       owl:ObjectProperty ;
      rdfs:domain npg:Publication ;
      rdfs:isDefinedBy npg: ;
      rdfs:range npg:XmlAsset ;
      skos:definition "The :hasXmlAsset property relates a publication to an xml-asset."@en ;
      skos:prefLabel "Has XML Asset"@en .

npg:hash
      a       owl:DatatypeProperty ;
      rdfs:isDefinedBy npg: ;
      rdfs:range rdfs:Literal ;
      skos:definition "The :hash property specifies a hash value over an entity URI used as a data integrity check."@en ;
      skos:prefLabel "Hash "@en .

npg:id
      a       owl:DatatypeProperty ;
      rdfs:isDefinedBy npg: ;
      rdfs:range rdfs:Literal ;
      skos:definition "The :id property provides a unique ID for a thing."@en ;
      skos:note "The :id value forms the local part of the full URI for an entity name."@en ;
      skos:prefLabel "ID"@en .

npg:idHash
      a       owl:DatatypeProperty ;
      rdfs:isDefinedBy npg: ;
      rdfs:range rdfs:Literal ;
      owl:deprecated "true"^^xsd:boolean ;
      skos:definition "The :idHash property specifies a string hash value for an ID."@en ;
      skos:prefLabel "ID Hash"@en .

npg:imageList
      a       owl:ObjectProperty ;
      rdfs:domain npg:Publication ;
      rdfs:isDefinedBy npg: ;
      rdfs:range rdf:List ;
      skos:definition "The :imageList property specifies an ordered list of images for a publication."@en ;
      skos:prefLabel "Image List"@en .

npg:isAssetOf
      a       owl:ObjectProperty ;
      rdfs:domain npg:Asset ;
      rdfs:isDefinedBy npg: ;
      rdfs:range npg:Publication ;
      owl:inverseOf npg:hasAsset ;
      skos:definition "The :isAssetOf property relates an asset to the publication it represents."@en ;
      skos:prefLabel "Is Asset Of"@en .

npg:isCorresponding
      a       owl:DatatypeProperty ;
      rdfs:domain npg:Contributor ;
      rdfs:isDefinedBy npg: ;
      rdfs:range xsd:boolean ;
      skos:definition "The :isCorresponding property marks whether a contributor is a corresponding author."@en ;
      skos:prefLabel "Is Corresponding"@en .

npg:isCurated
      a       owl:DatatypeProperty ;
      rdfs:domain npg:Image ;
      rdfs:isDefinedBy npg: ;
      rdfs:range xsd:boolean ;
      skos:definition "The :isCurated property marks whether an image is editiorially managed."@en ;
      skos:prefLabel "Is Curated"@en .

npg:isEventWorkflow
      a       owl:DatatypeProperty ;
      rdfs:domain npg:Publication ;
      rdfs:isDefinedBy npg: ;
      rdfs:range xsd:boolean ;
      skos:definition "The :isEventWorkflow property marks whether a publication is in the new metadata-based (event) workflow."@en ;
      skos:prefLabel "Is Event Workflow"@en .

npg:isGroup
      a       owl:DatatypeProperty ;
      rdfs:domain npg:Contributor ;
      rdfs:isDefinedBy npg: ;
      rdfs:range xsd:boolean ;
      skos:definition "The :isGroup property marks whether a contributor name refers to a collective agent, i.e. a group of people or an institution."@en ;
      skos:prefLabel "Is Group"@en .

npg:isIssueBased
      a       owl:DatatypeProperty ;
      rdfs:domain npg:Journal ;
      rdfs:isDefinedBy npg: ;
      rdfs:range xsd:boolean ;
      skos:definition "The :isIssueBased property marks whether a journal publishes issues."@en ;
      skos:prefLabel "Is Issue Based"@en .

npg:isLeaf
      a       owl:DatatypeProperty ;
      rdfs:domain npg:Type ;
      rdfs:isDefinedBy npg: ;
      rdfs:range xsd:boolean ;
      skos:definition "The :isLeaf property marks whether a SKOS concept is a leaf SKOS concept."@en ;
      skos:prefLabel "Is Leaf"@en .

npg:isNamedResource
      a       owl:AnnotationProperty ;
      rdfs:isDefinedBy npg: ;
      skos:definition "The :isNamedResource property marks whether an object resource is named or is unnamed (i.e. a blank node)."@en ;
      skos:prefLabel "Is Named Resource"@en .

npg:isPrimaryArticleType
      a       owl:DatatypeProperty ;
      rdfs:domain npg:ArticleType ;
      rdfs:isDefinedBy npg: ;
      rdfs:range xsd:boolean ;
      skos:definition "The :isPrimaryArticleType property marks whether an article-type can be used for grouping purposes."@en ;
      skos:prefLabel "Is PrimaryArticleType"@en .

npg:isPublishReady
      a       owl:DatatypeProperty ;
      rdfs:domain npg:Type ;
      rdfs:isDefinedBy npg: ;
      rdfs:range xsd:boolean ;
      skos:definition "The :isPublishReady property marks whether a type is ready for publishing."@en ;
      skos:prefLabel "Is Publish Ready"@en .

npg:isRepeatable
      a       owl:AnnotationProperty ;
      rdfs:isDefinedBy npg: ;
      skos:definition "The :isRepeatable property marks whether a property can be repeated."@en ;
      skos:prefLabel "Is Repeatable"@en .

npg:isRoot
      a       owl:DatatypeProperty ;
      rdfs:domain npg:Type ;
      rdfs:isDefinedBy npg: ;
      rdfs:range xsd:boolean ;
      skos:definition "The :isRoot property marks whether a SKOS concept is a SKOS top concept."@en ;
      skos:prefLabel "Is Root"@en .

npg:isTestInstance
      a       owl:DatatypeProperty ;
      rdfs:isDefinedBy npg: ;
      rdfs:range xsd:boolean ;
      skos:definition "The :isTestInstance property marks whether a resource is to be used for test purposes only."@en ;
      skos:prefLabel "Is Test Instance"@en .

npg:isVocabulary
      a       owl:AnnotationProperty ;
      rdfs:isDefinedBy npg: ;
      skos:definition "The :isVocabulary property marks whether a class is used for a controlled vocabulary."@en ;
      skos:prefLabel "Is Vocabulary"@en .

npg:issn
      a       owl:DatatypeProperty ;
      rdfs:domain npg:Serial ;
      rdfs:isDefinedBy npg: ;
      rdfs:range rdfs:Literal ;
      owl:equivalentProperty
              bibo:issn ;
      skos:definition "The :issn property specifies an ISSN number for a serial."@en ;
      skos:prefLabel "ISSN"@en .

npg:issue
      a       owl:DatatypeProperty ;
      rdfs:domain npg:Journal ;
      rdfs:isDefinedBy npg: ;
      rdfs:range rdfs:Literal ;
      owl:equivalentProperty
              bibo:issue ;
      skos:definition "The :issue property specifies an issue label for a journal."@en ;
      skos:prefLabel "Issue"@en .

npg:issueEnd
      a       owl:DatatypeProperty ;
      rdfs:domain npg:Serial ;
      rdfs:isDefinedBy npg: ;
      rdfs:range rdfs:Literal ;
      skos:definition "The :issueEnd property specifies the end issue for a serial publication."@en ;
      skos:prefLabel "Issue End"@en .

npg:issueStart
      a       owl:DatatypeProperty ;
      rdfs:domain npg:Serial ;
      rdfs:isDefinedBy npg: ;
      rdfs:range rdfs:Literal ;
      skos:definition "The :issueStart property specifies the start issue for a serial publication."@en ;
      skos:prefLabel "Issue Start"@en .

npg:itemList
      a       owl:ObjectProperty ;
      rdfs:domain npg:Collection ;
      rdfs:isDefinedBy npg: ;
      rdfs:range rdf:List ;
      skos:definition "The :itemList property specifies an ordered list of items."@en ;
      skos:prefLabel "Item List"@en .

npg:itemNumber
      a       owl:DatatypeProperty ;
      rdfs:domain npg:Item ;
      rdfs:isDefinedBy npg: ;
      rdfs:range xsd:integer ;
      skos:definition "The :itemNumber property specifies the number of an item within a collection."@en ;
      skos:prefLabel "Item Number"@en .

npg:itemReferenceList
      a       owl:ObjectProperty ;
      rdfs:domain npg:Collection ;
      rdfs:isDefinedBy npg: ;
      rdfs:range rdf:List ;
      skos:definition "The :itemReferenceList property specifies an ordered list of item references."@en ;
      skos:prefLabel "Item Reference List"@en .

npg:itemType
      a       owl:ObjectProperty ;
      rdfs:domain npg:Item ;
      rdfs:isDefinedBy npg: ;
      skos:definition "The :itemType property specifies the type of an item."@en ;
      skos:prefLabel "Item Type"@en .

npg:name
      a       owl:DatatypeProperty ;
      rdfs:domain npg:Contributor ;
      rdfs:isDefinedBy npg: ;
      rdfs:range rdfs:Literal ;
      owl:equivalentProperty
              foaf:name ;
      skos:definition "The :name property specifies the full name for a thing."@en ;
      skos:prefLabel "Name"@en .

npg:namespace
      a       owl:ObjectProperty ;
      rdfs:domain owl:Class ;
      rdfs:isDefinedBy npg: ;
      skos:definition "The :namespace property provides the RDF namespace used in creating instances of a class."@en ;
      skos:prefLabel "Namespace"@en .

npg:number
      a       owl:DatatypeProperty ;
      rdfs:domain npg:Component ;
      rdfs:isDefinedBy npg: ;
      rdfs:range xsd:integer ;
      skos:definition "The :number property specifies a sequence number for a component such as a figure."@en ;
      skos:prefLabel "Number"@en .

npg:orcid
      a       owl:ObjectProperty ;
      rdfs:domain npg:Publication ;
      rdfs:isDefinedBy npg: ;
      skos:definition "The :orcid property relates a publication to an ORCID record."@en ;
      skos:note "As we currently have no persons as such registered in our data model, we use the :orcid property with the :Contributor publication component that proxies for a person."@en ;
      skos:prefLabel "ORCID"@en .

npg:otherCode
      a       owl:DatatypeProperty ;
      rdfs:domain npg:Type ;
      rdfs:isDefinedBy npg: ;
      rdfs:range rdfs:Literal ;
      skos:definition "The :otherCode property specifies a number or string used by external applications as an ID for an entity."@en ;
      skos:prefLabel "Other Code"@en .

npg:pageEnd
      a       owl:DatatypeProperty ;
      rdfs:domain npg:Document ;
      rdfs:isDefinedBy npg: ;
      rdfs:range rdfs:Literal ;
      owl:equivalentProperty
              bibo:pageEnd ;
      skos:definition "The :pageEnd property specifies an ending page number for a document."@en ;
      skos:prefLabel "Page End"@en .

npg:pageStart
      a       owl:DatatypeProperty ;
      rdfs:domain npg:Document ;
      rdfs:isDefinedBy npg: ;
      rdfs:range rdfs:Literal ;
      owl:equivalentProperty
              bibo:pageStart ;
      skos:definition "The :pageStart property specifies a starting page number for a document."@en ;
      skos:prefLabel "Page Start"@en .

npg:pages
      a       owl:DatatypeProperty ;
      rdfs:domain npg:Document ;
      rdfs:isDefinedBy npg: ;
      rdfs:range rdfs:Literal ;
      owl:equivalentProperty
              bibo:pages ;
      skos:definition "The :pages property specifies a page range numbering for a document."@en ;
      skos:prefLabel "Pages"@en .

npg:publicationDate
      a       owl:DatatypeProperty ;
      rdfs:domain npg:Publication ;
      rdfs:isDefinedBy npg: ;
      rdfs:range xsd:date ;
      skos:definition "The :publicationDate property specifies the full date of a publication as a string."@en ;
      skos:prefLabel "Publication Date"@en .

npg:publicationDateTime
      a       owl:DatatypeProperty ;
      rdfs:domain npg:Publication ;
      rdfs:isDefinedBy npg: ;
      rdfs:range xsd:dateTime ;
      skos:definition "The :publicationDateTime property specifies the full date of a publication as a string, including the time of publication."@en ;
      skos:prefLabel "Publication DateTime"@en .

npg:publicationName
      a       owl:DatatypeProperty ;
      rdfs:domain npg:Publication ;
      rdfs:isDefinedBy npg: ;
      rdfs:range rdfs:Literal ;
      skos:definition "The :publicationName property specifies a string name for an external publication."@en ;
      skos:prefLabel "Publication Name"@en .

npg:publicationYear
      a       owl:DatatypeProperty ;
      rdfs:domain npg:Publication ;
      rdfs:isDefinedBy npg: ;
      rdfs:range xsd:gYear ;
      skos:definition "The :publicationYear property specifies the year date of a publication as a string."@en ;
      skos:prefLabel "Publication Year"@en .

npg:publicationYearMonth
      a       owl:DatatypeProperty ;
      rdfs:domain npg:Publication ;
      rdfs:isDefinedBy npg: ;
      rdfs:range xsd:gYearMonth ;
      skos:definition "The :publicationYearMonth property specifies the year and month date of a publication as a string."@en ;
      skos:prefLabel "Publication YearMonth"@en .

npg:relation
      a       owl:ObjectProperty ;
      rdfs:domain npg:Publication ;
      rdfs:isDefinedBy npg: ;
      rdfs:range npg:Publication ;
      skos:definition "The :relation property relates a publication to a publication."@en ;
      skos:prefLabel "Relation"@en .

npg:replacedBy
      a       owl:ObjectProperty ;
      rdfs:domain npg:Publication ;
      rdfs:isDefinedBy npg: ;
      rdfs:range npg:Publication ;
      owl:inverseOf npg:replaces ;
      skos:definition "The :replacedBy property relates a publication to another publication that replaces it."@en ;
      skos:prefLabel "Replaced By"@en .

npg:replaces
      a       owl:ObjectProperty ;
      rdfs:domain npg:Publication ;
      rdfs:isDefinedBy npg: ;
      rdfs:range npg:Publication ;
      owl:inverseOf npg:replacedBy ;
      skos:definition "The :replaces property relates a publication to another publication that it replaces."@en ;
      skos:prefLabel "Replaces"@en .

npg:repository
      a       owl:ObjectProperty ;
      rdfs:domain npg:Asset ;
      rdfs:isDefinedBy npg: ;
      skos:definition "The :repository property relates an asset to a storage repository."@en ;
      skos:prefLabel "Repository"@en .

npg:repositoryId
      a       owl:DatatypeProperty ;
      rdfs:domain npg:Asset ;
      rdfs:isDefinedBy npg: ;
      rdfs:range rdfs:Literal ;
      skos:definition "The :repositoryId property specifies a (local) repository ID for an asset."@en ;
      skos:prefLabel "Repository ID"@en .

npg:sectionLevel
      a       owl:DatatypeProperty ;
      rdfs:domain npg:Section ;
      rdfs:isDefinedBy npg: ;
      rdfs:range xsd:integer ;
      skos:definition "The :sectionLevel property specifies the level number of a section."@en ;
      skos:prefLabel "Section Level"@en .

npg:shortTitle
      a       owl:DatatypeProperty ;
      rdfs:domain npg:Publication ;
      rdfs:isDefinedBy npg: ;
      rdfs:range rdfs:Literal ;
      owl:equivalentProperty
              bibo:shortTitle ;
      skos:definition "The :shortTitle property specifies an abbreviated title for a publication."@en ;
      skos:prefLabel "Short Title"@en .

npg:sortLetter
      a       owl:DatatypeProperty ;
      rdfs:domain npg:Type ;
      rdfs:isDefinedBy npg: ;
      rdfs:range rdfs:Literal ;
      skos:definition "The :sortLetter property specifies the initial letter of an entity name to facilitate sort operations."@en ;
      skos:note "This property is generally computed from a build-time rule."@en ;
      skos:prefLabel "Sort Letter"@en .

npg:sortNumber
      a       owl:DatatypeProperty ;
      rdfs:domain npg:Type ;
      rdfs:isDefinedBy npg: ;
      rdfs:range xsd:integer ;
      skos:definition "The :sortLetter property specifies the sequence number of an entity to facilitate sort operations."@en ;
      skos:prefLabel "Sort Number"@en .

npg:status
      a       owl:DatatypeProperty ;
      rdfs:isDefinedBy npg: ;
      rdfs:range rdfs:Literal ;
      skos:definition "The :status property specifies a status string for an ontology term."@en ;
      skos:prefLabel "Status"@en .

npg:subjectPath
      a       owl:DatatypeProperty ;
      rdfs:domain npg:Journal ;
      rdfs:isDefinedBy npg: ;
      rdfs:range rdfs:Literal ;
      skos:definition "The :subjectPath property specifies the position of a term within the subjects taxonomy by providing a path with the IDs of its successors."@en ;
      skos:prefLabel "Subject Path"@en .

npg:test
      a       owl:DatatypeProperty ;
      rdfs:isDefinedBy npg: ;
      skos:definition "The :test property specifies a general string test property."@en ;
      skos:prefLabel "Test"@en .

npg:timestamp
      a       owl:DatatypeProperty ;
      rdfs:isDefinedBy npg: ;
      rdfs:range rdfs:Literal ;
      skos:definition "The :timestamp property specifies a generic timestamp for an object."@en ;
      skos:prefLabel "Timestamp"@en .

npg:title
      a       owl:DatatypeProperty ;
      rdfs:domain npg:Publication ;
      rdfs:isDefinedBy npg: ;
      rdfs:range rdfs:Literal ;
      skos:definition "The :title property specifies a title to the main body content of a publication as a string."@en ;
      skos:prefLabel "Title"@en .

npg:titleXml
      a       owl:DatatypeProperty ;
      rdfs:domain npg:Publication ;
      rdfs:isDefinedBy npg: ;
      rdfs:range rdfs:Literal ;
      skos:definition "The :titleXml property specifies a title to the main body content of a publication as an XML string."@en ;
      skos:prefLabel "Title (XML)"@en .

npg:treeDepth
      a       owl:DatatypeProperty ;
      rdfs:domain npg:Type ;
      rdfs:isDefinedBy npg: ;
      rdfs:range xsd:integer ;
      skos:definition "The :treeDepth property specifies the depth of a term within a taxonomy tree."@en ;
      skos:note "This property is generally computed by a build-time rule"@en ;
      skos:prefLabel "Tree Depth"@en .

npg:type
      a       owl:AnnotationProperty ;
      rdfs:isDefinedBy npg: ;
      skos:definition "The :type property specifies the local name of the graph namespace used for instances of a class."@en ;
      skos:note "This property is used as a surrogate for the class name. There is a one-to-one relation between the class name and its associated graph, e.g. instances of the class :Subject are assigned to the subjects: graph."@en ;
      skos:prefLabel "Type"@en .

npg:volume
      a       owl:DatatypeProperty ;
      rdfs:domain npg:Journal ;
      rdfs:isDefinedBy npg: ;
      rdfs:range rdfs:Literal ;
      owl:equivalentProperty
              bibo:volume ;
      skos:definition "The :volume property specifies a volume label for a journal."@en ;
      skos:prefLabel "Volume"@en .

npg:volumeEnd
      a       owl:DatatypeProperty ;
      rdfs:domain npg:Serial ;
      rdfs:isDefinedBy npg: ;
      rdfs:range rdfs:Literal ;
      skos:definition "The :issueEnd property specifies the end volume for a serial publication."@en ;
      skos:prefLabel "Volume End"@en .

npg:volumeStart
      a       owl:DatatypeProperty ;
      rdfs:domain npg:Serial ;
      rdfs:isDefinedBy npg: ;
      rdfs:range rdfs:Literal ;
      skos:definition "The :issueEnd property specifies the start volume for a serial publication."@en ;
      skos:prefLabel "Volume Start"@en .

npg:webpage
      a       owl:ObjectProperty ;
      rdfs:domain npg:Publication ;
      rdfs:isDefinedBy npg: ;
      owl:equivalentProperty
              foaf:page ;
      skos:definition "The :webpage property relates a publication to a page on the web that describes it."@en ;
      skos:prefLabel "Web Page"@en .

npg:xmlId
      a       owl:DatatypeProperty ;
      rdfs:isDefinedBy npg: ;
      rdfs:range rdfs:Literal ;
      skos:definition "The :xmlId property specifies an ID assigned to an XML element."@en ;
      skos:prefLabel "XML ID"@en .

npg:year
      a       owl:DatatypeProperty ;
      rdfs:domain npg:Event ;
      rdfs:isDefinedBy npg: ;
      rdfs:range xsd:gYear ;
      skos:definition "The :date property specifies the year date of an event as a string."@en ;
      skos:prefLabel "Year"@en .

npg:yearMonth
      a       owl:DatatypeProperty ;
      rdfs:domain npg:Event ;
      rdfs:isDefinedBy npg: ;
      rdfs:range xsd:gYearMonth ;
      skos:definition "The :date property specifies the year and month date of an event as a string."@en ;
      skos:prefLabel "YearMonth"@en .
      


mo:Arranger a owl:Class ;
  rdfs:label "arranger" ;
  mo:level "2" ;
  rdfs:subClassOf foaf:Agent ;
  owl:equivalentClass [ a owl:Restriction ;
          owl:onProperty event:isAgentIn ;
          owl:someValuesFrom mo:Arrangement ] ;
  vs:term_status "unstable" .

mo:CD a owl:Class ;
  rdfs:label "CD" ;
  mo:level "1" ;
  rdfs:comment "Compact Disc used as medium to record a musical manifestation." ;
  rdfs:isDefinedBy mo: ;
  rdfs:subClassOf mo:Medium ;
  vs:term_status "unstable" .

mo:Composer a owl:Class ;
  rdfs:label "composer" ;
  mo:level "2" ;
  rdfs:subClassOf foaf:Agent ;
  owl:equivalentClass [ a owl:Restriction ;
          owl:onProperty event:isAgentIn ;
          owl:someValuesFrom mo:Composition ] ;
  vs:term_status "unstable" .

mo:Conductor a owl:Class ;
  rdfs:label "conductor" ;
  mo:level "2" ;
  rdfs:subClassOf foaf:Agent ;
  owl:equivalentClass [ a owl:Restriction ;
          owl:onProperty mo:conducted ;
          owl:someValuesFrom mo:Performance ] ;
  vs:term_status "unstable" .

mo:DAT a owl:Class ;
  rdfs:label "DAT" ;
  mo:level "1" ;
  rdfs:comment "Digital Audio Tape used as medium to record a musical manifestation." ;
  rdfs:isDefinedBy mo: ;
  rdfs:subClassOf mo:Medium ;
  vs:term_status "unstable" .

mo:DCC a owl:Class ;
  rdfs:label "DCC" ;
  mo:level "1" ;
  rdfs:comment "Digital Compact Cassette used as medium to record a musical manifestation." ;
  rdfs:isDefinedBy mo: ;
  rdfs:subClassOf mo:Medium ;
  vs:term_status "unstable" .

mo:DVDA a owl:Class ;
  rdfs:label "DVDA" ;
  mo:level "1" ;
  rdfs:comment "DVD-Audio used as medium to record a musical manifestation." ;
  rdfs:isDefinedBy mo: ;
  rdfs:subClassOf mo:Medium ;
  vs:term_status "unstable" .

mo:ED2K a owl:Class ;
  rdfs:label "ED2K" ;
  mo:level "1" ;
  rdfs:comment "Something available on the E-Donkey peer-2-peer filesharing network" ;
  rdfs:isDefinedBy mo: ;
  rdfs:subClassOf mo:Medium ;
  vs:term_status "unstable" .

mo:Festival a owl:Class ;
  rdfs:label "Festival" ;
  mo:level "2" ;
  rdfs:comment """
      A festival - musical/artistic event lasting several days, like Glastonbury, Rock Am Ring...
      We migth decompose this event (which is in fact just a classification of the space/time region related to 
      a particular festival) using hasSubEvent in several performances at different space/time.
  """ ;
  rdfs:isDefinedBy mo: ;
  rdfs:subClassOf event:Event ;
  vs:term_status "stable" .

mo:Instrumentation a owl:Class ;
  rdfs:label "instrumentation" ;
  mo:level "2" ;
  rdfs:comment """
      Instrumentation deals with the techniques of writing music for a specific instrument, 
      including the limitations of the instrument, playing techniques and idiomatic handling of the instrument.
  """ ;
  rdfs:isDefinedBy mo: ;
  rdfs:subClassOf mo:Arrangement ;
  vs:term_status "stable" .

mo:Libretto a owl:Class ;
  rdfs:label "libretto" ;
  mo:level "2" ;
  rdfs:comment """
              Libretto
      """ ;
  rdfs:isDefinedBy mo: ;
  rdfs:subClassOf mo:MusicalExpression ;
  vs:term_status "stable" .

mo:Listener a owl:Class ;
  rdfs:label "listened" ;
  mo:level "2" ;
  rdfs:subClassOf foaf:Agent ;
  owl:equivalentClass [ a owl:Restriction ;
          owl:onProperty mo:listened ;
          owl:someValuesFrom mo:Performance ] ;
  vs:term_status "unstable" .

mo:MD a owl:Class ;
  rdfs:label "MD" ;
  mo:level "1" ;
  rdfs:comment "Mini Disc used as medium to record a musical manifestation." ;
  rdfs:isDefinedBy mo: ;
  rdfs:subClassOf mo:Medium ;
  vs:term_status "unstable" .

mo:MagneticTape a owl:Class ;
  rdfs:label "MagneticTape" ;
  mo:level "1" ;
  rdfs:comment "Magnetic analogue tape used as medium to record a musical manifestation." ;
  rdfs:isDefinedBy mo: ;
  rdfs:subClassOf mo:Medium ;
  vs:term_status "unstable" .

mo:Orchestration a owl:Class ;
  rdfs:label "orchestration" ;
  mo:level "2" ;
  rdfs:comment """
          Orchestration includes, in addition to instrumentation, the handling of groups of instruments and their balance and interaction.
  """ ;
  rdfs:isDefinedBy mo: ;
  rdfs:subClassOf mo:Arrangement ;
  vs:term_status "stable" .

mo:Performer a owl:Class ;
  rdfs:label "performer" ;
  mo:level "2" ;
  rdfs:subClassOf foaf:Agent ;
  owl:equivalentClass [ a owl:Restriction ;
          owl:onProperty mo:performed ;
          owl:someValuesFrom mo:Performance ] ;
  vs:term_status "unstable" .

mo:SACD a owl:Class ;
  rdfs:label "SACD" ;
  mo:level "1" ;
  rdfs:comment "Super Audio Compact Disc used as medium to record a musical manifestation." ;
  rdfs:isDefinedBy mo: ;
  rdfs:subClassOf mo:Medium ;
  vs:term_status "unstable" .

mo:Show a owl:Class ;
  rdfs:label "Show" ;
  mo:level "2" ;
  rdfs:comment """
      A show - a musical event lasting several days, in a particular venue. Examples can be
      "The Magic Flute" at the Opera Bastille, August 2005, or a musical in the west end...
  """ ;
  rdfs:isDefinedBy mo: ;
  rdfs:subClassOf event:Event ;
  vs:term_status "stable" .

mo:SoloMusicArtist a owl:Class ;
  rdfs:label "solo music artist" ;
  mo:level "1" ;
  rdfs:comment "Single person whose musical creative work shows sensitivity and imagination." ;
  rdfs:isDefinedBy mo: ;
  rdfs:subClassOf mo:MusicArtist,
      foaf:Person ;
  vs:term_status "stable" .

mo:SoundEngineer a owl:Class ;
  rdfs:label "sound engineer" ;
  mo:level "2" ;
  rdfs:subClassOf foaf:Agent ;
  owl:equivalentClass [ a owl:Restriction ;
          owl:onProperty mo:engineered ;
          owl:someValuesFrom mo:Performance ] ;
  vs:term_status "unstable" .

mo:Stream a owl:Class ;
  rdfs:label "Stream" ;
  mo:level "1" ;
  rdfs:comment "Transmission over a network  used as medium to broadcast a musical manifestation" ;
  rdfs:isDefinedBy mo: ;
  rdfs:subClassOf mo:Medium ;
  vs:term_status "unstable" .

mo:Torrent a owl:Class ;
  rdfs:label "Torrent" ;
  mo:level "1" ;
  rdfs:comment "Something available on the Bittorrent peer-2-peer filesharing network" ;
  rdfs:isDefinedBy mo: ;
  rdfs:subClassOf mo:Medium ;
  vs:term_status "unstable" .

mo:Transcription a owl:Class ;
  rdfs:label "transcription" ;
  mo:level "2" ;
  rdfs:comment "Transcription event" ;
  rdfs:isDefinedBy mo: ;
  rdfs:subClassOf event:Event ;
  vs:term_status "testing" .

mo:Vinyl a owl:Class ;
  rdfs:label "Vinyl" ;
  mo:level "1" ;
  rdfs:comment "Vinyl used as medium to record a musical manifestation" ;
  rdfs:isDefinedBy mo: ;
  rdfs:subClassOf mo:Medium ;
  vs:term_status "unstable" .

mo:activity a owl:ObjectProperty ;
  rdfs:label "activity" ;
  mo:level "1" ;
  rdfs:comment "Relates an artist to an activity period" ;
  rdfs:domain mo:MusicArtist ;
  rdfs:isDefinedBy mo: ;
  rdfs:range mo:Activity ;
  vs:term_status "testing" .

mo:activity_end a owl:DatatypeProperty ;
  rdfs:label "activity end" ;
  mo:level "1" ;
  rdfs:comment "Relates an artist to a date at which its activity ended" ;
  rdfs:domain mo:MusicArtist ;
  rdfs:isDefinedBy mo: ;
  rdfs:range xsd:date ;
  vs:term_status "testing" .

mo:activity_start a owl:DatatypeProperty ;
  rdfs:label "activity start" ;
  mo:level "1" ;
  rdfs:comment "Relates an artist to a date at which its activity started" ;
  rdfs:domain mo:MusicArtist ;
  rdfs:isDefinedBy mo: ;
  rdfs:range xsd:date ;
  vs:term_status "testing" .

mo:album a mo:ReleaseType ;
  dc:description """
      One or more track issued together.
          This is a type of MusicalManifestation defined by the musical industry.
  """ ;
  dc:title "album" ;
  mo:level "1" ;
  rdfs:isDefinedBy mo: .

mo:amazon_asin a owl:ObjectProperty ;
  rdfs:label "amazon_asin" ;
  mo:level "1" ;
  rdfs:comment "Used to link a work or the expression of a work to its corresponding Amazon ASINs page." ;
  rdfs:domain [ a owl:Class ;
          owl:unionOf ( frbr:Work frbr:Expression frbr:Manifestation frbr:Item ) ] ;
  rdfs:isDefinedBy mo: ;
  rdfs:range foaf:Document ;
  rdfs:subPropertyOf foaf:isPrimaryTopicOf ;
  vs:term_status "stable" .

mo:artist a owl:ObjectProperty ;
  rdfs:label "artist" ;
  mo:level "1" ;
  rdfs:comment "Relates a membership event with the corresponding artist" ;
  rdfs:domain mo:Membership ;
  rdfs:isDefinedBy mo: ;
  rdfs:range foaf:Agent ;
  vs:term_status "testing" .

mo:audiobook a mo:ReleaseType ;
  dc:description """
      Book read by a narrator without music.
      This is a type of MusicalManifestation defined by the musical industry.
  """ ;
  dc:title "audio book" ;
  mo:level "1" ;
  rdfs:isDefinedBy mo: .

mo:availableAs a owl:ObjectProperty ;
  owl:equivalentProperty mo:available_as ;
  vs:term_status "deprecated" .

mo:biography a owl:ObjectProperty ;
  rdfs:label "biography" ;
  mo:level "1" ;
  rdfs:comment "Used to link an artist to their online biography." ;
  rdfs:domain mo:MusicArtist ;
  rdfs:isDefinedBy mo: ;
  rdfs:range foaf:Document ;
  rdfs:subPropertyOf foaf:isPrimaryTopicOf ;
  vs:term_status "stable" .

mo:bitsPerSample a owl:DatatypeProperty,
      owl:FunctionalProperty ;
  mo:level "1" ;
  rdfs:comment """
      Associates a digital signal to the number a bits used to encode one sample. Range is xsd:int.
  """ ;
  rdfs:domain mo:DigitalSignal ;
  rdfs:isDefinedBy mo: ;
  rdfs:range xsd:int ;
  vs:term_status "stable" .

mo:bootleg a mo:ReleaseStatus ;
  dc:description "An unofficial/underground musical work or the expression of a musical work that was not sanctioned by the artist and/or the corporate body. " ;
  dc:title "bootleg" ;
  mo:level "1" ;
  rdfs:isDefinedBy mo: .

mo:bpm a owl:DatatypeProperty ;
  rdfs:label "bpm" ;
  mo:level "2" ;
  rdfs:comment """
      Indicates the BPM of a MusicalWork or a particular Performance 
      Beats per minute: the pace of music measured by the number of beats occurring in 60 seconds.
  """ ;
  rdfs:domain [ a owl:Class ;
          owl:unionOf ( mo:MusicalWork mo:Performance mo:Signal ) ] ;
  rdfs:isDefinedBy mo: ;
  rdfs:range xsd:float ;
  vs:term_status "stable" .

mo:catalogue_number a owl:DatatypeProperty ;
  rdfs:label "catalogue number" ;
  mo:level "1" ;
  rdfs:comment "Links a release with the corresponding catalogue number" ;
  rdfs:domain mo:Release ;
  rdfs:isDefinedBy mo: ;
  rdfs:range xsd:string ;
  rdfs:subPropertyOf mo:uuid ;
  vs:term_status "testing" .

mo:channels a owl:DatatypeProperty,
      owl:FunctionalProperty ;
  mo:level "1" ;
  rdfs:comment """
      Associates a signal to the number of channels it holds (mono --> 1, stereo --> 2). Range is xsd:int.
  """ ;
  rdfs:domain mo:Signal ;
  rdfs:isDefinedBy mo: ;
  rdfs:range xsd:int ;
  vs:term_status "stable" .

mo:collaborated_with a owl:ObjectProperty,
      owl:SymmetricProperty ;
  rdfs:label "collaborated_with" ;
  mo:level "1" ;
  rdfs:comment "Used to relate two collaborating people on a work." ;
  rdfs:domain foaf:Agent ;
  rdfs:isDefinedBy mo: ;
  rdfs:range foaf:Agent ;
  vs:term_status "unstable" .

mo:compilation a mo:ReleaseType ;
  dc:description """
      Collection of previously released manifestations of a musical expression by one or more artists.
      This is a type of MusicalManifestation defined by the musical industry.
  """ ;
  dc:title "compilation" ;
  mo:level "1" ;
  rdfs:isDefinedBy mo: .

mo:compilation_of a owl:ObjectProperty ;
  rdfs:label "compilation_of" ;
  mo:level "1" ;
  rdfs:comment "Indicates that a musical manifestation is a compilation of several Signals." ;
  rdfs:domain mo:MusicalManifestation ;
  rdfs:isDefinedBy mo: ;
  rdfs:range mo:Signal ;
  vs:term_status "unstable" .

mo:composer a owl:ObjectProperty ;
  rdfs:label "composer" ;
  mo:level "2" ;
  rdfs:comment """
      Associates a composition event to the actual composer. For example,
      this property could link the event corresponding to the composition of the
      Magic Flute in 1782 to Mozart himself (who obviously has a FOAF profile:-) ).
  """ ;
  rdfs:domain mo:Composition ;
  rdfs:isDefinedBy mo: ;
  rdfs:range foaf:Agent ;
  rdfs:subPropertyOf event:agent ;
  vs:term_status "stable" .

mo:contains_sample_from a owl:ObjectProperty ;
  rdfs:label "contains_sample_from" ;
  mo:level "1" ;
  rdfs:comment """
      Relates a signal to another signal, which has been sampled.
      """ ;
  rdfs:isDefinedBy mo: ;
  rdfs:subPropertyOf mo:derived_from ;
  vs:term_status "unstable" .

mo:discography a owl:ObjectProperty ;
  rdfs:label "discography" ;
  mo:level "1" ;
  rdfs:comment "Used to links an artist to an online discography of their musical works. The discography should provide a summary of each released musical work of the artist." ;
  rdfs:domain mo:MusicArtist ;
  rdfs:isDefinedBy mo: ;
  rdfs:range foaf:Document ;
  rdfs:subPropertyOf foaf:isPrimaryTopicOf ;
  vs:term_status "stable" .

mo:discogs a owl:ObjectProperty ;
  rdfs:label "discogs" ;
  mo:level "1" ;
  rdfs:comment "Used to link a musical work or the expression of a musical work, an artist or a corporate body to to its corresponding Discogs page." ;
  rdfs:domain [ a owl:Class ;
          owl:unionOf ( mo:MusicalWork mo:MusicalExpression mo:MusicalManifestation mo:MusicArtist mo:CorporateBody ) ] ;
  rdfs:isDefinedBy mo: ;
  rdfs:range foaf:Document ;
  rdfs:subPropertyOf foaf:isPrimaryTopicOf ;
  vs:term_status "stable" .

mo:djmix_of a owl:ObjectProperty ;
  rdfs:label "djmix_of" ;
  mo:level "1" ;
  rdfs:comment """Indicates that all (or most of) the tracks of a musical work or the expression of a musical work were mixed together from all (or most of) the tracks from another musical work or the expression of a musical work to form a so called DJ-Mix. 

The tracks might have been altered by pitching (so that the tempo of one track matches the tempo of the following track) and fading (so that one track blends in smoothly with the other). If the tracks have been more substantially altered, the "mo:remix" relationship type is more appropriate. """ ;
  rdfs:isDefinedBy mo: ;
  rdfs:subPropertyOf mo:derived_from ;
  vs:term_status "unstable" .

mo:duration a owl:DatatypeProperty ;
  mo:level "1" ;
  rdfs:comment "The duration of a track or a signal in ms" ;
  rdfs:domain [ a owl:Class ;
          owl:unionOf ( mo:Track mo:Signal ) ] ;
  rdfs:isDefinedBy mo: ;
  rdfs:range xsd:float ;
  vs:term_status "testing" .

mo:ean a owl:DatatypeProperty ;
  rdfs:label "ean" ;
  mo:level "1" ;
  rdfs:comment "The European Article Number (EAN) is a universal identifier for products, commonly printed in form of barcodes on them. The numbers represented by those codes can either be 8 or 13 digits long, with the 13-digit-version being most common. EANs form a superset of the North American Universal Product Code (UPC) as every UPC can be made an EAN by adding a leading zero to it. Additionally every EAN is also a Japanese Article Number (JAN). The identifiers were formerly assigned by EAN International which merged with Uniform Code Council (UCC, the guys behind the UPCs) and Electronic Commerce Council of Canada (ECCC) to become GS1. " ;
  rdfs:domain mo:Release ;
  rdfs:isDefinedBy mo: ;
  rdfs:range xsd:string ;
  rdfs:subPropertyOf mo:gtin ;
  vs:term_status "testing" .

mo:encodes a owl:ObjectProperty ;
  rdfs:label "encodes" ;
  mo:level "1" ;
  rdfs:comment """
      Relates a MusicalItem (a track on a particular CD, an audio file, a stream somewhere) to the signal it encodes.

      This is usually a lower-resolution version of the master signal (issued from a Recording event).
  """ ;
  rdfs:domain mo:MusicalItem ;
  rdfs:isDefinedBy mo: ;
  rdfs:range mo:Signal ;
  vs:term_status "unstable" .

mo:encoding a owl:DatatypeProperty ;
  rdfs:label "encoding" ;
  mo:level "1" ;
  rdfs:comment "Method used to convert analog electronic signals into digital format such as \"MP3 CBR @ 128kbps\", \"OGG @ 160kbps\", \"FLAC\", etc." ;
  rdfs:domain mo:AudioFile ;
  rdfs:isDefinedBy mo: ;
  rdfs:range rdfs:Literal ;
  vs:term_status "unstable" .

mo:ep a mo:ReleaseType ;
  dc:description """
          An EP
  """ ;
  dc:title "ep" ;
  mo:level "1" ;
  rdfs:isDefinedBy mo: .

mo:eventHomePage a owl:ObjectProperty ;
  owl:equivalentProperty mo:event_homepage ;
  vs:term_status "deprecated" .

mo:exchange_item a owl:ObjectProperty ;
  rdfs:label "exchange_item" ;
  mo:level "1" ;
  rdfs:comment "A person, a group of person or an organization exchanging an exemplar of a single manifestation." ;
  rdfs:domain foaf:Agent ;
  rdfs:isDefinedBy mo: ;
  rdfs:range frbr:Item ;
  vs:term_status "stable" .

mo:fanpage a owl:ObjectProperty ;
  rdfs:label "fanpage" ;
  mo:level "1" ;
  rdfs:comment "Used to link an artist to a fan-created webpage devoted to that artist." ;
  rdfs:domain mo:MusicArtist ;
  rdfs:isDefinedBy mo: ;
  rdfs:range foaf:Document ;
  rdfs:subPropertyOf foaf:isPrimaryTopicOf ;
  vs:term_status "stable" .

mo:freedownload a owl:ObjectProperty ;
  rdfs:isDefinedBy mo: ;
  owl:equivalentProperty mo:free_download ;
  vs:term_status "deprecated" .

mo:genre a owl:ObjectProperty ;
  rdfs:label "genre" ;
  mo:level "2" ;
  rdfs:comment """
      Associates an event (like a performance or a recording) to a particular musical genre.
      Further version of this property may also include works and scores in the domain.
  """ ;
  rdfs:domain [ a owl:Class ;
          owl:unionOf ( foaf:Agent mo:Performance mo:Arrangement mo:Composition mo:Recording mo:RecordingSession mo:MusicalWork mo:MusicalExpression mo:MusicalManifestation mo:MusicalItem ) ] ;
  rdfs:isDefinedBy mo: ;
  rdfs:range mo:Genre ;
  rdfs:subPropertyOf ao:genre ;
  vs:term_status "stable" .

mo:grid a owl:DatatypeProperty ;
  rdfs:label "GRid" ;
  mo:level "1" ;
  rdfs:comment "The Global Release Identifier (GRid) is a system for uniquely identifying Releases of music over electronic networks (that is, online stores where you can buy music as digital files). As that it can be seen as the equivalent of the BarCode (or more correctly the GTIN) as found on physical releases of music. Like the ISRC (a code for identifying single recordings as found on releases) it was developed by the IFPI but it does not appear to be a standard of the ISO." ;
  rdfs:domain mo:Release ;
  rdfs:isDefinedBy mo: ;
  rdfs:range xsd:string ;
  rdfs:subPropertyOf mo:uuid ;
  vs:term_status "testing" .

mo:group a owl:ObjectProperty ;
  rdfs:label "group" ;
  mo:level "1" ;
  rdfs:comment "Relates a membership event with the corresponding group" ;
  rdfs:domain mo:Membership ;
  rdfs:isDefinedBy mo: ;
  rdfs:range foaf:Group ;
  vs:term_status "testing" .

mo:has_track a owl:ObjectProperty ;
  rdfs:isDefinedBy mo: ;
  owl:equivalentProperty mo:track ;
  vs:term_status "deprecated" .

mo:headliner a owl:ObjectProperty ;
  rdfs:label "headliner" ;
  mo:level "2" ;
  rdfs:comment "Relates a performance to the headliner(s) involved" ;
  rdfs:isDefinedBy mo: ;
  rdfs:subPropertyOf mo:performer ;
  vs:term_status "testing" .

mo:homepage a owl:ObjectProperty ;
  rdfs:label "homepage" ;
  mo:level "1" ;
  rdfs:comment "Links an artist, a record, etc. to a corresponding web page" ;
  rdfs:domain [ a owl:Class ;
          owl:unionOf ( mo:MusicalWork mo:MusicArtist mo:MusicalExpression mo:MusicalManifestation mo:MusicalItem ) ] ;
  rdfs:isDefinedBy mo: ;
  rdfs:range foaf:Document ;
  rdfs:subPropertyOf foaf:isPrimaryTopicOf ;
  vs:term_status "stable" .

mo:image a owl:ObjectProperty ;
  rdfs:label "image" ;
  mo:level "1" ;
  rdfs:comment "Indicates a pictorial image (JPEG, GIF, PNG, Etc.) of a musical work, the expression of a musical work, the manifestation of a work or the examplar of a manifestation." ;
  rdfs:domain [ a owl:Class ;
          owl:unionOf ( mo:MusicalWork mo:MusicArtist mo:MusicalExpression mo:MusicalManifestation mo:MusicalItem ) ] ;
  rdfs:isDefinedBy mo: ;
  rdfs:range foaf:Image ;
  rdfs:subPropertyOf foaf:depiction ;
  vs:term_status "stable" .

mo:imdb a owl:ObjectProperty ;
  rdfs:label "imdb" ;
  mo:level "1" ;
  rdfs:comment "Used to link an artist, a musical work or the expression of a musical work to their equivalent page on IMDb, the InternetMovieDatabase." ;
  rdfs:domain [ a owl:Class ;
          owl:unionOf ( mo:MusicalWork mo:MusicalExpression mo:MusicalManifestation mo:MusicArtist mo:CorporateBody ) ] ;
  rdfs:isDefinedBy mo: ;
  rdfs:range foaf:Document ;
  rdfs:subPropertyOf foaf:isPrimaryTopicOf ;
  vs:term_status "stable" .

mo:instrument a owl:ObjectProperty ;
  mo:level "2" ;
  rdfs:comment "Relates a performance to a musical instrument involved" ;
  rdfs:domain mo:Performance ;
  rdfs:isDefinedBy mo: ;
  rdfs:range mo:Instrument ;
  rdfs:subPropertyOf event:factor ;
  vs:term_status "stable" .

mo:interview a mo:ReleaseType ;
  dc:description """
      Recording of the questioning of a person.
      This is a type of MusicalManifestation defined by the musical industry.
  """ ;
  dc:title "interview" ;
  mo:level "1" ;
  rdfs:isDefinedBy mo: .

mo:ipi a owl:DatatypeProperty ;
  rdfs:label "ipi" ;
  mo:level "1" ;
  rdfs:comment "The Interested Parties Information Code (IPI) is an ISO standard similar to ISBNs for identifying the people or groups with some involvement with a particular musical work / compositions." ;
  rdfs:domain mo:MusicArtist ;
  rdfs:isDefinedBy mo: ;
  rdfs:range xsd:string ;
  rdfs:subPropertyOf mo:uuid ;
  vs:term_status "testing" .

mo:ismn a owl:DatatypeProperty ;
  rdfs:label "ismn" ;
  mo:level "1" ;
  rdfs:comment "The International Standard Music Number (ISMN) is an ISO standard similar to ISBNs for identifying printed music publications" ;
  rdfs:domain [ a owl:Class ;
          owl:unionOf ( mo:PublishedLyrics mo:PublishedLibretto mo:PublishedScore ) ] ;
  rdfs:isDefinedBy mo: ;
  rdfs:range xsd:string ;
  rdfs:subPropertyOf mo:uuid ;
  vs:term_status "testing" .

mo:isrc a owl:DatatypeProperty ;
  rdfs:label "isrc" ;
  mo:level "1" ;
  rdfs:comment """
  The ISRC (International Standard Recording Code) is the international identification system for sound recordings and music videorecordings. 
  Each ISRC is a unique and permanent identifier for a specific recording which can be permanently encoded into a product as its digital fingerprint. 
  Encoded ISRC provide the means to automatically identify recordings for royalty payments.
  """ ;
  rdfs:domain mo:Signal ;
  rdfs:isDefinedBy mo: ;
  rdfs:range xsd:string ;
  rdfs:subPropertyOf mo:uuid ;
  vs:term_status "stable" .

mo:iswc a owl:DatatypeProperty ;
  rdfs:label "iswc" ;
  mo:level "1" ;
  rdfs:comment "Links a musical work to the corresponding ISWC number" ;
  rdfs:domain mo:MusicalWork ;
  rdfs:isDefinedBy mo: ;
  rdfs:range xsd:string ;
  rdfs:subPropertyOf mo:uuid ;
  vs:term_status "testing" .

mo:item a owl:ObjectProperty ;
  mo:level "1" ;
  rdfs:comment """
              Relates a musical manifestation to a musical item (this album, and my particular cd) holding the
              entire manifestation, and not just a part of it.
      """ ;
  rdfs:domain mo:MusicalManifestation ;
  rdfs:isDefinedBy mo: ;
  rdfs:range mo:MusicalItem ;
  rdfs:subPropertyOf mo:available_as ;
  vs:term_status "testing" .

mo:key a owl:ObjectProperty ;
  rdfs:label "key" ;
  mo:level "2" ;
  rdfs:comment """
      Indicated the key used by the musicians during a performance, or the key of a MusicalWork.
      Any of 24 major or minor diatonic scales that provide the tonal framework for a piece of music.""" ;
  rdfs:domain [ a owl:Class ;
          owl:unionOf ( mo:MusicalWork mo:Performance mo:Signal ) ] ;
  rdfs:isDefinedBy mo: ;
  rdfs:range keys:Key ;
  vs:term_status "stable" .

mo:label a owl:ObjectProperty ;
  rdfs:label "label" ;
  mo:level "1" ;
  rdfs:comment "Associates a release event with the label releasing the record" ;
  rdfs:domain [ a owl:Class ;
          owl:unionOf ( mo:Release mo:MusicArtist ) ] ;
  rdfs:isDefinedBy mo: ;
  rdfs:range mo:Label ;
  vs:term_status "testing" .

mo:lc a owl:DatatypeProperty ;
  rdfs:label "lc" ;
  mo:level "1" ;
  rdfs:comment "The Label Code (LC) was introduced in 1977 by the IFPI (International Federation of Phonogram and Videogram Industries) in order to unmistakably identify the different record labels (see Introduction, Record labels) for rights purposes. The Label Code consists historically of 4 figures, presently being extended to 5 figures, preceded by LC and a dash (e.g. LC-0193 = Electrola; LC-0233 = His Master's Voice). Note that the number of countries using the LC is limited, and that the code given on the item is not always accurate." ;
  rdfs:domain mo:Label ;
  rdfs:isDefinedBy mo: ;
  rdfs:range xsd:string ;
  rdfs:subPropertyOf mo:uuid ;
  vs:term_status "testing" .

mo:level a owl:AnnotationProperty ;
  rdfs:label "level" ;
  rdfs:comment """
      This annotation property associates to a particular Music Ontology term the corresponding
      expressiveness level. These levels can be:

          - 1: Only editorial/Musicbrainz type information
          - 2: Workflow information
          - 3: Even decomposition

      This property is mainly used for specification generation.
  """ ;
  rdfs:isDefinedBy mo: .

mo:licence a owl:ObjectProperty ;
  rdfs:label "licence" ;
  mo:level "1" ;
  rdfs:comment """Used to link a work or the expression of a work to the license under which they can be manipulated (downloaded, modified, etc). 

This is usually used to link to a Creative Commons licence.""" ;
  rdfs:domain [ a owl:Class ;
          owl:unionOf ( frbr:Work frbr:Expression frbr:Manifestation ) ] ;
  rdfs:isDefinedBy mo: ;
  rdfs:range cc:License ;
  vs:term_status "stable" .

mo:live a mo:ReleaseType ;
  dc:description """
      A musical manifestation that was recorded live.
      This is a type of MusicalManifestation defined by the musical industry.""" ;
  dc:title "live" ;
  mo:level "1" ;
  rdfs:isDefinedBy mo: .

mo:lyrics a owl:ObjectProperty ;
  rdfs:label "lyrics" ;
  mo:level "2" ;
  rdfs:comment "Associates lyrics with a musical work" ;
  rdfs:domain mo:MusicalWork ;
  rdfs:isDefinedBy mo: ;
  rdfs:range mo:Lyrics ;
  vs:term_status "testing" .

mo:mailorder a owl:ObjectProperty ;
  rdfs:label "mailorder" ;
  mo:level "1" ;
  rdfs:comment "Used to link a musical work or the expression of a musical work to a website where people can buy a copy of the musical manifestation." ;
  rdfs:domain [ a owl:Class ;
          owl:unionOf ( frbr:Manifestation mo:MusicArtist mo:CorporateBody ) ] ;
  rdfs:isDefinedBy mo: ;
  rdfs:range foaf:Document ;
  rdfs:subPropertyOf foaf:isPrimaryTopicOf ;
  vs:term_status "stable" .

mo:mashup_of a owl:ObjectProperty ;
  rdfs:label "mashup_of" ;
  mo:level "1" ;
  rdfs:comment """Indicates that musical works or the expressions of a musical work were mashed up on this album or track. 

This means that two musical works or the expressions of a musical work by different artists are mixed together, over each other, or otherwise combined into a single musical work (usually by a third artist, the remixer).""" ;
  rdfs:isDefinedBy mo: ;
  rdfs:subPropertyOf mo:derived_from ;
  vs:term_status "unstable" .

mo:media_type a owl:ObjectProperty ;
  rdfs:label "has media type" ;
  mo:level "1" ;
  rdfs:comment "The mediatype (file format or MIME type, or physical medium) of a musical manifestation, e.g. a MP3, CD or vinyl." ;
  rdfs:domain mo:MusicalManifestation ;
  rdfs:isDefinedBy mo: ;
  rdfs:range dcterms:MediaType ;
  rdfs:subPropertyOf dcterms:format ;
  vs:term_status "testing" .

mo:medley_of a owl:ObjectProperty ;
  rdfs:label "medley_of" ;
  mo:level "1" ;
  rdfs:comment """Indicates that a musical expression is a medley of several other musical expressions. 

This means that the orignial musical expression were rearranged to create a new musical expression in the form of a medley. """ ;
  rdfs:isDefinedBy mo: ;
  rdfs:subPropertyOf mo:derived_from ;
  vs:term_status "unstable" .

mo:member a owl:ObjectProperty ;
  rdfs:label "member" ;
  mo:level "1" ;
  rdfs:comment """
      Indicates a member of a musical group
  """ ;
  rdfs:domain mo:MusicGroup ;
  rdfs:isDefinedBy mo: ;
  rdfs:range foaf:Agent ;
  rdfs:subPropertyOf foaf:member ;
  vs:term_status "stable" .

mo:member_of a owl:ObjectProperty ;
  rdfs:label "member_of" ;
  mo:level "1" ;
  rdfs:comment "Inverse of the foaf:member property" ;
  rdfs:domain foaf:Agent ;
  rdfs:isDefinedBy mo: ;
  rdfs:range foaf:Group ;
  owl:inverseOf foaf:member ;
  vs:term_status "unstable" .

mo:membership a owl:ObjectProperty ;
  rdfs:label "membership" ;
  mo:level "1" ;
  rdfs:comment "Relates an agent with related membership events" ;
  rdfs:domain foaf:Agent ;
  rdfs:isDefinedBy mo: ;
  rdfs:range mo:Membership ;
  vs:term_status "testing" .

mo:meter a owl:DatatypeProperty ;
  rdfs:label "meter" ;
  mo:level "2" ;
  rdfs:comment "Associates a musical work or a score with its meter" ;
  rdfs:domain [ a owl:Class ;
          owl:unionOf ( mo:MusicalWork mo:Score ) ] ;
  rdfs:isDefinedBy mo: ;
  vs:term_status "testing" .

mo:movement a owl:ObjectProperty ;
  rdfs:label "has_movement" ;
  mo:level "2" ;
  rdfs:comment "Indicates that a musical work has movements" ;
  rdfs:domain mo:MusicalWork ;
  rdfs:isDefinedBy mo: ;
  rdfs:range mo:Movement ;
  vs:term_status "unstable" .

mo:movementNum a owl:DatatypeProperty ;
  owl:equivalentProperty mo:movement_number .

mo:musicbrainz a owl:ObjectProperty ;
  rdfs:label "musicbrainz" ;
  mo:level "1" ;
  rdfs:comment """
      Linking an agent, a track or a record to its corresponding Musicbrainz page.
      """ ;
  rdfs:domain [ a owl:Class ;
          owl:unionOf ( mo:MusicalWork mo:MusicalManifestation foaf:Agent mo:Signal ) ] ;
  rdfs:isDefinedBy mo: ;
  rdfs:range foaf:Document ;
  rdfs:subPropertyOf foaf:isPrimaryTopicOf ;
  vs:term_status "stable" .

mo:musicbrainz_guid a owl:DatatypeProperty ;
  rdfs:label "Musicbrainz GUID" ;
  mo:level "1" ;
  rdfs:comment "Links an object to the corresponding Musicbrainz identifier" ;
  rdfs:domain [ a owl:Class ;
          owl:unionOf ( mo:MusicArtist mo:Track mo:Record mo:SignalGroup mo:Signal mo:ReleaseEvent mo:Label ) ] ;
  rdfs:isDefinedBy mo: ;
  rdfs:subPropertyOf mo:uuid ;
  vs:term_status "testing" .

mo:musicmoz a owl:ObjectProperty ;
  rdfs:label "musicmoz" ;
  mo:level "1" ;
  rdfs:comment "Used to link an artist, a musical work or the expression of a musical work to its corresponding MusicMoz page." ;
  rdfs:domain [ a owl:Class ;
          owl:unionOf ( mo:MusicArtist mo:MusicalWork mo:MusicalExpression mo:MusicalManifestation ) ] ;
  rdfs:isDefinedBy mo: ;
  rdfs:range foaf:Document ;
  rdfs:subPropertyOf foaf:isPrimaryTopicOf ;
  vs:term_status "stable" .

mo:myspace a owl:ObjectProperty ;
  rdfs:label "myspace" ;
  mo:level "1" ;
  rdfs:comment "Used to link a person to its corresponding MySpace page." ;
  rdfs:domain foaf:Agent ;
  rdfs:isDefinedBy mo: ;
  rdfs:range foaf:Document ;
  rdfs:subPropertyOf foaf:isPrimaryTopicOf ;
  vs:term_status "stable" .

mo:official a mo:ReleaseStatus ;
  dc:description "Any musical work or the expression of a musical work officially sanctioned by the artist and/or their corporate body." ;
  dc:title "official" ;
  mo:level "1" ;
  rdfs:isDefinedBy mo: .

mo:olga a owl:ObjectProperty ;
  rdfs:label "olga" ;
  mo:level "1" ;
  rdfs:comment "Used to link a track to a tabulature file for track in the On-Line Guitar Archive." ;
  rdfs:domain mo:Track ;
  rdfs:isDefinedBy mo: ;
  rdfs:range foaf:Document ;
  rdfs:subPropertyOf foaf:isPrimaryTopicOf ;
  vs:term_status "stable" .

mo:onlinecommunity a owl:ObjectProperty ;
  rdfs:label "onlinecommunity" ;
  mo:level "1" ;
  rdfs:comment "Used to link a person with an online community web page like a blog, a wiki, a forum, a livejournal page, Etc." ;
  rdfs:domain foaf:Agent ;
  rdfs:isDefinedBy mo: ;
  rdfs:range foaf:Document ;
  rdfs:subPropertyOf foaf:isPrimaryTopicOf ;
  vs:term_status "stable" .

mo:opus a owl:DatatypeProperty ;
  rdfs:label "opus" ;
  mo:level "2" ;
  rdfs:comment """
      Used to define a creative work, especially a musical composition numbered to designate the order of a composer's works.
  """ ;
  rdfs:domain mo:MusicalWork ;
  rdfs:isDefinedBy mo: ;
  rdfs:range rdfs:Literal ;
  vs:term_status "stable" .

mo:origin a owl:ObjectProperty ;
  rdfs:label "origin" ;
  mo:level "1" ;
  rdfs:comment "Relates an artist to its geographic origin" ;
  rdfs:domain mo:MusicArtist ;
  rdfs:isDefinedBy mo: ;
  rdfs:range geo:SpatialThing ;
  vs:term_status "testing" .

mo:other_release_of a owl:ObjectProperty,
      owl:SymmetricProperty ;
  rdfs:label "other_release_of" ;
  mo:level "1" ;
  rdfs:comment "Indicates that two musical manifestations are essentially the same." ;
  rdfs:domain mo:MusicalManifestation ;
  rdfs:isDefinedBy mo: ;
  rdfs:range mo:MusicalManifestation ;
  vs:term_status "unstable" .

mo:paiddownload a owl:ObjectProperty ;
  rdfs:isDefinedBy mo: ;
  owl:equivalentProperty mo:paid_download ;
  vs:term_status "deprecated" .

mo:possess_item a owl:ObjectProperty ;
  rdfs:label "possess_item" ;
  mo:level "1" ;
  rdfs:comment "A person, a group of person or an organization possessing an exemplar of a single manifestation." ;
  rdfs:domain foaf:Agent ;
  rdfs:isDefinedBy mo: ;
  rdfs:range frbr:Item ;
  vs:term_status "stable" .

mo:preview a owl:ObjectProperty ;
  mo:level "1" ;
  rdfs:comment """
              Relates a musical manifestation to a musical item (this album, and my particular cd), which holds
              a preview of the manifestation (eg. one track for an album, or a snippet for a track)
      """ ;
  rdfs:domain mo:MusicalManifestation ;
  rdfs:isDefinedBy mo: ;
  rdfs:range mo:MusicalItem ;
  rdfs:subPropertyOf mo:available_as ;
  vs:term_status "testing" .

mo:preview_download a owl:ObjectProperty ;
  rdfs:label "preview download" ;
  mo:level "1" ;
  rdfs:comment """
              This property can be used to link from a person to the website where they make previews of their works available, or from
              a manifestation (a track or an album, for example) to a web page where a preview download is available.

              This property MUST be used only if the content is just available through a web page (holding, for example
              a Flash application) - it is better to link to actual content directly through the use of mo:available_as and
              mo:Stream, mo:Torrent or mo:ED2K, etc. Therefore, Semantic Web user agents that don't know how to read HTML and even
              less to rip streams from Flash applications can still access the audio content.
      """ ;
  rdfs:domain [ a owl:Class ;
          owl:unionOf ( frbr:Manifestation foaf:Agent mo:CorporateBody ) ] ;
  rdfs:isDefinedBy mo: ;
  rdfs:range foaf:Document ;
  rdfs:subPropertyOf mo:download,
      foaf:isPrimaryTopicOf ;
  vs:term_status "stable" .

mo:primary_instrument a owl:ObjectProperty ;
  rdfs:label "primary instrument" ;
  mo:level "1" ;
  rdfs:comment "Indicates that an artist primarily plays an instrument, or that a member was primarily playing a particular instrument during his membership" ;
  rdfs:domain [ a owl:Class ;
          owl:unionOf ( mo:Membership foaf:Agent ) ] ;
  rdfs:isDefinedBy mo: ;
  rdfs:range mo:Instrument ;
  vs:term_status "testing" .

mo:produced_score a owl:ObjectProperty ;
  rdfs:label "produced score" ;
  mo:level "2" ;
  rdfs:comment """
      Associates an arrangement event to a score product (score here does not refer to a published score, but more
      an abstract arrangement of a particular work).
  """ ;
  rdfs:domain mo:Arrangement ;
  rdfs:isDefinedBy mo: ;
  rdfs:range mo:Score ;
  rdfs:subPropertyOf event:product ;
  vs:term_status "unstable" .

mo:produced_signal_group a owl:ObjectProperty ;
  rdfs:label "produced signal group" ;
  mo:level "2" ;
  rdfs:comment "Associates a recording session with a group of master signals produced by it." ;
  rdfs:domain mo:RecordingSession ;
  rdfs:isDefinedBy mo: ;
  rdfs:range mo:SignalGroup ;
  rdfs:subPropertyOf event:product ;
  vs:term_status "testing" .

mo:producesSignal a owl:ObjectProperty ;
  rdfs:isDefinedBy mo: ;
  owl:equivalentProperty mo:produced_signal ;
  vs:term_status "deprecated" .

mo:producesSound a owl:ObjectProperty ;
  rdfs:isDefinedBy mo: ;
  owl:equivalentProperty mo:produced_sound ;
  vs:term_status "deprecated" .

mo:producesWork a owl:ObjectProperty ;
  owl:equivalentProperty mo:produced_work .

mo:productOfComposition a owl:ObjectProperty ;
  rdfs:isDefinedBy mo: ;
  owl:equivalentProperty mo:composed_in ;
  vs:term_status "deprecated" .

mo:promotion a mo:ReleaseStatus ;
  dc:description "A giveaway musical work or the expression of a musical work intended to promote an upcoming official musical work or the expression of a musical work." ;
  dc:title "promotion" ;
  mo:level "1" ;
  rdfs:isDefinedBy mo: .

mo:publicationOf a owl:ObjectProperty ;
  owl:equivalentProperty mo:publication_of ;
  vs:term_status "deprecated" .

mo:publishedAs a owl:ObjectProperty ;
  owl:equivalentProperty mo:published_as ;
  vs:term_status "deprecated" .

mo:publishingLocation a owl:ObjectProperty ;
  owl:equivalentProperty mo:publishing_location ;
  vs:term_status "deprecated" .

mo:puid a owl:DatatypeProperty ;
  rdfs:label "puid" ;
  mo:level "1" ;
  rdfs:comment """
      Link a signal to the PUIDs associated with it, that is, PUID computed from MusicalItems (mo:AudioFile) 
      derived from this signal.
      PUIDs (Portable Unique IDentifier) are the IDs used in the 
      proprietary MusicDNS AudioFingerprinting system which is operated by MusicIP.

      Using PUIDs, one (with some luck) can identify the Signal object associated with a particular audio file, therefore allowing
      to access further information (on which release this track is featured? etc.). Using some more metadata one can identify
      the particular Track corresponding to the audio file (a track on a particular release).""" ;
  rdfs:domain mo:Signal ;
  rdfs:isDefinedBy mo: ;
  rdfs:range xsd:string ;
  vs:term_status "stable" .

mo:record a owl:ObjectProperty ;
  rdfs:label "released record" ;
  mo:level "1" ;
  rdfs:comment "Associates a release with the records it contains. A single release can be associated with multiple records, for example for a multi-disc release." ;
  rdfs:domain mo:Release ;
  rdfs:isDefinedBy mo: ;
  rdfs:range mo:Record ;
  vs:term_status "testing" .

mo:record_count a owl:DatatypeProperty ;
  rdfs:label "record count" ;
  mo:level "1" ;
  rdfs:comment "Associates a release with the number of records it contains, e.g. the number of discs it contains in the case of a multi-disc release." ;
  rdfs:domain mo:Release ;
  rdfs:isDefinedBy mo: ;
  rdfs:range xsd:int ;
  vs:term_status "testing" .

mo:record_number a owl:DatatypeProperty ;
  rdfs:label "has record number" ;
  mo:level "1" ;
  rdfs:comment "Indicates the position of a record in a release (e.g. a 2xLP, etc.)." ;
  rdfs:domain mo:Record ;
  rdfs:isDefinedBy mo: ;
  rdfs:range xsd:nonNegativeInteger ;
  vs:term_status "testing" .

mo:record_side a owl:DatatypeProperty ;
  rdfs:label "has record side" ;
  mo:level "1" ;
  rdfs:comment """Associates the side on a vinyl record, where a track is located, e.g. A, B, C, etc. This property can then also be used 
in conjunction with mo:track_number, so that one can infer e.g. "A1", that means, track number 1 on side A.""" ;
  rdfs:domain mo:Track ;
  rdfs:isDefinedBy mo: ;
  rdfs:range xsd:string ;
  vs:term_status "testing" .

mo:release a owl:ObjectProperty ;
  rdfs:label "release" ;
  mo:level "1" ;
  rdfs:comment "Associates a release with the corresponding release event" ;
  rdfs:domain mo:ReleaseEvent ;
  rdfs:isDefinedBy mo: ;
  rdfs:range mo:Release ;
  rdfs:subPropertyOf event:product ;
  vs:term_status "testing" .

mo:releaseStatus a owl:ObjectProperty ;
  owl:equivalentProperty mo:release_status ;
  vs:term_status "deprecated" .

mo:releaseType a owl:ObjectProperty ;
  owl:equivalentProperty mo:release_type ;
  vs:term_status "deprecated" .

mo:remaster_of a owl:ObjectProperty ;
  rdfs:label "remaster_of" ;
  mo:level "1" ;
  rdfs:comment """This relates two musical work or the expression of a musical work, where one is a remaster of the other. 

A remaster is a new version made for release from source recordings that were earlier released separately. This is usually done to improve the audio quality or adjust for more modern playback equipment. The process generally doesn't involve changing the music in any artistically important way. It may, however, result in tracks that are a few seconds longer or shorter.""" ;
  rdfs:isDefinedBy mo: ;
  rdfs:subPropertyOf mo:derived_from ;
  vs:term_status "unstable" .

mo:remix a mo:ReleaseType ;
  dc:description """
      Musical manifestation that primarily contains remixed material. 
      This is a type of MusicalManifestation defined by the musical industry.
  """ ;
  dc:title "remix" ;
  mo:level "1" ;
  rdfs:isDefinedBy mo: .

mo:remix_of a owl:ObjectProperty ;
  rdfs:label "remix_of" ;
  mo:level "1" ;
  rdfs:comment "Used to relate the remix of a musical work in a substantially altered version produced by mixing together individual tracks or segments of an original musical source work." ;
  rdfs:isDefinedBy mo: ;
  rdfs:subPropertyOf mo:derived_from ;
  vs:term_status "unstable" .

mo:review a owl:ObjectProperty ;
  rdfs:label "review" ;
  mo:level "1" ;
  rdfs:comment """Used to link a work or the expression of a work to a review. 

The review does not have to be open content, as long as it is accessible to the general internet population.""" ;
  rdfs:domain [ a owl:Class ;
          owl:unionOf ( frbr:Work frbr:Expression frbr:Manifestation ) ] ;
  rdfs:isDefinedBy mo: ;
  rdfs:range foaf:Document ;
  rdfs:subPropertyOf foaf:isPrimaryTopicOf ;
  vs:term_status "stable" .

mo:sampleRate a owl:DatatypeProperty ;
  owl:equivalentProperty mo:sample_rate ;
  vs:term_status "deprecated" .

mo:sampledVersionOf a owl:ObjectProperty ;
  rdfs:isDefinedBy mo: ;
  owl:equivalentProperty mo:sampled_version_of ;
  vs:term_status "deprecated" .

mo:sell_item a owl:ObjectProperty ;
  rdfs:label "sell_item" ;
  mo:level "1" ;
  rdfs:comment "A person, a group of person or an organization selling an exemplar of a single manifestation." ;
  rdfs:domain foaf:Agent ;
  rdfs:isDefinedBy mo: ;
  rdfs:range frbr:Item ;
  vs:term_status "stable" .

mo:signal a owl:ObjectProperty ;
  rdfs:label "signal" ;
  mo:level "1" ;
  rdfs:comment "Associates a group of signals with one of the signals it contains" ;
  rdfs:domain mo:SignalGroup ;
  rdfs:isDefinedBy mo: ;
  rdfs:range mo:Signal ;
  vs:term_status "testing" .

mo:signalTime a owl:ObjectProperty ;
  rdfs:isDefinedBy mo: ;
  owl:equivalentProperty mo:time ;
  vs:term_status "deprecated" .

mo:similar_to a owl:ObjectProperty ;
  rdfs:label "similar_to" ;
  mo:level "1" ;
  rdfs:comment """
          A similarity relationships between two objects (so far, either an agent, a signal or a genre, but
      this could grow).
      This relationship is pretty general and doesn't make any assumptions on how the similarity claim
      was derived.
      Such similarity statements can come from a range of different sources (Musicbrainz similarities between
      artists, or coming from some automatic content analysis).
      However, the origin of such statements should be kept using a named graph approach - and ultimately, the 
      documents providing such statements should attach some metadata to themselves (confidence of the claim, etc.).
      """ ;
  rdfs:domain [ a owl:Class ;
          owl:unionOf ( foaf:Agent mo:MusicalWork mo:MusicalExpression mo:MusicalManifestation mo:MusicalItem mo:Genre ) ] ;
  rdfs:isDefinedBy mo: ;
  rdfs:range [ a owl:Class ;
          owl:unionOf ( foaf:Agent mo:MusicalWork mo:MusicalExpression mo:MusicalManifestation mo:MusicalItem mo:Genre ) ] ;
  vs:term_status "unstable" .

mo:singer a owl:ObjectProperty ;
  mo:level "2" ;
  rdfs:comment "Relates a performance to an involved singer" ;
  rdfs:domain mo:Performance ;
  rdfs:isDefinedBy mo: ;
  rdfs:range foaf:Agent ;
  rdfs:subPropertyOf mo:performer ;
  vs:term_status "stable" .

mo:single a mo:ReleaseType ;
  dc:description "A single or record single is a type of release, typically a recording of two tracks. In most cases, the single is a song that is released separately from an album, but it can still appear on an album." ;
  dc:title "single" ;
  mo:level "1" ;
  rdfs:isDefinedBy mo: .

mo:soundtrack a mo:ReleaseType ;
  dc:description """
      Sound recording on a narrow strip of a motion picture film.
      This is a type of MusicalManifestation defined by the musical industry.
  """ ;
  dc:title "soundtrack" ;
  mo:level "1" ;
  rdfs:isDefinedBy mo: .

mo:spokenword a mo:ReleaseType ;
  dc:description """
      Spoken word is a form of music or artistic performance in which lyrics, poetry, or stories are spoken rather than sung. 
      Spoken-word is often done with a musical background, but emphasis is kept on the speaker.
      This is a type of MusicalManifestation defined by the musical industry.
  """ ;
  dc:title "spoken word" ;
  mo:level "1" ;
  rdfs:isDefinedBy mo: .

mo:supporting_musician a owl:ObjectProperty ;
  rdfs:label "supporting_musician" ;
  mo:level "1" ;
  rdfs:comment "Used to relate an artist doing long-time instrumental or vocal support for another artist." ;
  rdfs:domain mo:MusicArtist ;
  rdfs:isDefinedBy mo: ;
  rdfs:range mo:MusicArtist ;
  vs:term_status "unstable" .

mo:tempo a owl:DatatypeProperty ;
  rdfs:label "tempo" ;
  mo:level "2" ;
  rdfs:comment """
      Rate of speed or pace of music. Tempo markings are traditionally given in Italian; 
      common markings include: grave (solemn; very, very slow); largo (broad; very slow); 
      adagio (quite slow); andante (a walking pace); moderato (moderate); allegro (fast; cheerful); 
      vivace (lively); presto (very fast); accelerando (getting faster); ritardando (getting slower); 
      and a tempo (in time; returning to the original pace).
  """ ;
  rdfs:domain [ a owl:Class ;
          owl:unionOf ( mo:MusicalWork mo:Performance mo:Signal ) ] ;
  rdfs:isDefinedBy mo: ;
  rdfs:range xsd:string ;
  vs:term_status "stable" .

mo:text a owl:DatatypeProperty ;
  rdfs:label "text" ;
  mo:level "2" ;
  rdfs:comment "Associates lyrics with their text." ;
  rdfs:domain mo:Lyrics ;
  rdfs:isDefinedBy mo: ;
  vs:term_status "testing" .

mo:trackNum a owl:DatatypeProperty ;
  rdfs:isDefinedBy mo: ;
  owl:equivalentProperty mo:track_number ;
  vs:term_status "deprecated" .

mo:track_count a owl:DatatypeProperty ;
  rdfs:label "track count" ;
  mo:level "1" ;
  rdfs:comment "The track count of a record" ;
  rdfs:domain mo:Record ;
  rdfs:isDefinedBy mo: ;
  rdfs:range xsd:int ;
  vs:term_status "testing" .

mo:translation_of a owl:ObjectProperty ;
  rdfs:label "translation_of" ;
  mo:level "1" ;
  rdfs:comment "Indicates that a work or the expression of a work has translated or transliterated into another expression of a work." ;
  rdfs:domain frbr:Expression ;
  rdfs:isDefinedBy mo: ;
  rdfs:range frbr:Expression ;
  vs:term_status "unstable" .

mo:tribute_to a owl:ObjectProperty ;
  rdfs:label "tribute_to" ;
  mo:level "1" ;
  rdfs:comment "Indicates a musical work or the expression of a musical work that is a tribute to an artist - normally consisting of music being composed by the artist but performed by other artists. " ;
  rdfs:domain mo:MusicalManifestation ;
  rdfs:isDefinedBy mo: ;
  rdfs:range mo:MusicArtist ;
  vs:term_status "unstable" .

mo:trmid a owl:DatatypeProperty ;
  rdfs:label "trmid" ;
  mo:level "1" ;
  rdfs:comment """
      Indicates the TRMID of a track.
      TRM IDs are MusicBrainz' old AudioFingerprinting system. 
      TRM (TRM Recognizes Music) IDs are (somewhat) unique ids that represent 
      the audio signature of a musical piece (see AudioFingerprint).
  """ ;
  rdfs:domain mo:Signal ;
  rdfs:isDefinedBy mo: ;
  rdfs:range xsd:string ;
  vs:term_status "stable" .

mo:upc a owl:DatatypeProperty ;
  rdfs:label "upc" ;
  mo:level "1" ;
  rdfs:comment "UPC stands for \"Universal Product Code\", which was the original barcode used in the United States and Canada. The UPC (now officially EAN.UCC-12 is a numerical method of identifying products without redundancy worldwide for all types of products in the retail sector. The EAN is a superset of the original UPC increasing the digits to 13 with the prefix 0 reserved for UPC. As of 2005, manufacturers are only allowed to use the new 13-digit codes on their items, rather than having two separate numbers." ;
  rdfs:domain mo:Release ;
  rdfs:isDefinedBy mo: ;
  rdfs:range xsd:string ;
  rdfs:subPropertyOf mo:gtin ;
  vs:term_status "testing" .

mo:usedInPerformance a owl:ObjectProperty ;
  rdfs:isDefinedBy mo: ;
  owl:equivalentProperty mo:performed_in ;
  vs:term_status "deprecated" .

mo:usedInRecording a owl:ObjectProperty ;
  rdfs:isDefinedBy mo: ;
  owl:equivalentProperty mo:recorded_in ;
  vs:term_status "deprecated" .

mo:usesSound a owl:ObjectProperty ;
  rdfs:isDefinedBy mo: ;
  owl:equivalentProperty mo:recording_of ;
  vs:term_status "deprecated" .

mo:usesWork a owl:ObjectProperty ;
  rdfs:isDefinedBy mo: ;
  owl:equivalentProperty mo:performance_of ;
  vs:term_status "deprecated" .

mo:want_item a owl:ObjectProperty ;
  rdfs:label "want_item" ;
  mo:level "1" ;
  rdfs:comment "A person, a group of person or an organization wanting an exemplar of a single manifestation." ;
  rdfs:domain foaf:Agent ;
  rdfs:isDefinedBy mo: ;
  rdfs:range frbr:Item ;
  vs:term_status "stable" .

mo:wikipedia a owl:ObjectProperty ;
  rdfs:label "wikipedia" ;
  mo:level "1" ;
  rdfs:comment """
      Used to link an work, an expression of a work, a manifestation of a work, 
      a person, an instrument or a musical genre to its corresponding WikiPedia page. 
      The full URL should be used, not just the WikiName.
  """ ;
  rdfs:domain [ a owl:Class ;
          owl:unionOf ( frbr:Work frbr:Expression frbr:Manifestation frbr:Item foaf:Agent mo:Instrument mo:Genre ) ] ;
  rdfs:isDefinedBy mo: ;
  rdfs:range foaf:Document ;
  rdfs:subPropertyOf foaf:isPrimaryTopicOf ;
  vs:term_status "stable" .

vs:term_status a owl:AnnotationProperty .

mo:Activity a owl:Class ;
  rdfs:label "activity" ;
  mo:level "1" ;
  rdfs:comment """
      An activity period, defining when an artist was musically active.
  """ ;
  rdfs:isDefinedBy mo: ;
  rdfs:subClassOf event:Event ;
  vs:term_status "testing" .

mo:AudioFile a owl:Class ;
  rdfs:label "audio file" ;
  mo:level "1" ;
  rdfs:comment "An audio file, which may be available on a local file system or through http, ftp, etc." ;
  rdfs:isDefinedBy mo: ;
  rdfs:subClassOf mo:Medium,
      foaf:Document ;
  vs:term_status "unstable" .

mo:MusicGroup a owl:Class ;
  rdfs:label "music group" ;
  mo:level "1" ;
  rdfs:comment "Group of musicians, or musical ensemble, usually popular or folk, playing parts of or improvising off of a musical arrangement. " ;
  rdfs:isDefinedBy mo: ;
  rdfs:subClassOf mo:MusicArtist,
      foaf:Group ;
  vs:term_status "stable" .

mo:PublishedLibretto a owl:Class ;
  rdfs:label "published libretto" ;
  mo:level "2" ;
  rdfs:comment "A published libretto" ;
  rdfs:isDefinedBy mo: ;
  rdfs:subClassOf mo:MusicalManifestation ;
  vs:term_status "stable" .

mo:PublishedLyrics a owl:Class ;
  rdfs:label "published lyrics" ;
  mo:level "2" ;
  rdfs:comment "Published lyrics, as a book or as a text file, for example" ;
  rdfs:isDefinedBy mo: ;
  rdfs:subClassOf mo:MusicalManifestation ;
  vs:term_status "stable" .

mo:PublishedScore a owl:Class ;
  rdfs:label "published score" ;
  mo:level "2" ;
  rdfs:comment "A published score (subclass of MusicalManifestation)" ;
  rdfs:isDefinedBy mo: ;
  rdfs:subClassOf mo:MusicalManifestation ;
  vs:term_status "stable" .

mo:arranged_in a owl:ObjectProperty ;
  rdfs:label "arranged in" ;
  mo:level "2" ;
  rdfs:comment """
      Associates a work to an arrangement event where it was arranged
  """ ;
  rdfs:domain mo:MusicalWork ;
  rdfs:isDefinedBy mo: ;
  rdfs:range mo:Arrangement ;
  rdfs:subPropertyOf event:isFactorOf ;
  owl:inverseOf mo:arrangement_of ;
  vs:term_status "unstable" .

mo:arrangement_of a owl:ObjectProperty ;
  rdfs:label "arrangement of" ;
  mo:level "2" ;
  rdfs:comment """
              Associates an arrangement event to a work
      """ ;
  rdfs:domain mo:Arrangement ;
  rdfs:isDefinedBy mo: ;
  rdfs:range mo:MusicalWork ;
  rdfs:subPropertyOf event:factor ;
  owl:inverseOf mo:arranged_in ;
  vs:term_status "unstable" .

mo:compiled a owl:ObjectProperty ;
  rdfs:label "compiled" ;
  mo:level "1" ;
  rdfs:comment "Used to relate an person or a group of person who compiled the manifestation of a musical work." ;
  rdfs:domain mo:MusicArtist ;
  rdfs:isDefinedBy mo: ;
  rdfs:range mo:MusicalManifestation ;
  owl:inverseOf mo:compiler ;
  vs:term_status "unstable" .

mo:compiler a owl:ObjectProperty ;
  rdfs:label "compiler" ;
  mo:level "1" ;
  rdfs:comment "Used to relate the manifestation of a musical work to a person or a group of person who compiled it." ;
  rdfs:domain mo:MusicalManifestation ;
  rdfs:isDefinedBy mo: ;
  rdfs:range mo:MusicArtist ;
  owl:inverseOf mo:compiled ;
  vs:term_status "unstable" .

mo:conductor a owl:ObjectProperty ;
  mo:level "2" ;
  rdfs:comment "Relates a performance to the conductor involved" ;
  rdfs:domain mo:Performance ;
  rdfs:isDefinedBy mo: ;
  rdfs:range foaf:Agent ;
  rdfs:subPropertyOf event:agent ;
  owl:inverseOf mo:conducted ;
  vs:term_status "stable" .

mo:djmixed a owl:ObjectProperty ;
  rdfs:label "djmixed" ;
  mo:level "1" ;
  rdfs:comment """Used to relate an artist who djmixed a musical work or the expression of a musical work. 

The artist usually selected the tracks, chose their sequence, and slightly changed them by fading (so that one track blends in smoothly with the other) or pitching (so that the tempo of one track matches the tempo of the following track). This applies to a 'Mixtape' in which all tracks were DJ-mixed together into one single long track. """ ;
  rdfs:domain mo:MusicArtist ;
  rdfs:isDefinedBy mo: ;
  rdfs:range mo:Signal ;
  owl:inverseOf mo:djmixed_by ;
  vs:term_status "unstable" .

mo:djmixed_by a owl:ObjectProperty ;
  rdfs:label "djmixed_by" ;
  mo:level "1" ;
  rdfs:comment """Used to relate a work or the expression of a work to an artist who djmixed it. 

The artist usually selected the tracks, chose their sequence, and slightly changed them by fading (so that one track blends in smoothly with the other) or pitching (so that the tempo of one track matches the tempo of the following track). This applies to a 'Mixtape' in which all tracks were DJ-mixed together into one single long track. """ ;
  rdfs:domain mo:Signal ;
  rdfs:isDefinedBy mo: ;
  rdfs:range mo:MusicArtist ;
  owl:inverseOf mo:djmixed ;
  vs:term_status "unstable" .

mo:engineer a owl:ObjectProperty ;
  mo:level "2" ;
  rdfs:comment "Relates a performance or a recording to the engineer involved" ;
  rdfs:domain [ a owl:Class ;
          owl:unionOf ( mo:Performance mo:Recording mo:RecordingSession ) ] ;
  rdfs:isDefinedBy mo: ;
  rdfs:range foaf:Agent ;
  rdfs:subPropertyOf event:agent ;
  owl:inverseOf mo:engineered ;
  vs:term_status "stable" .

mo:event_homepage a owl:ObjectProperty ;
  rdfs:label "event homepage" ;
  mo:level "2" ;
  rdfs:comment "Links a particular event to a web page" ;
  rdfs:domain event:Event ;
  rdfs:isDefinedBy mo: ;
  rdfs:range foaf:Document ;
  rdfs:subPropertyOf foaf:isPrimaryTopicOf ;
  vs:term_status "stable" .

mo:free_download a owl:ObjectProperty ;
  rdfs:label "free download" ;
  mo:level "1" ;
  rdfs:comment """
      This property can be used to link from a person to the website where they make their works available, or from
      a manifestation (a track or an album, for example) to a web page where it is available for free 
      download.

      This property MUST be used only if the content is just available through a web page (holding, for example
      a Flash application) - it is better to link to actual content directly through the use of mo:available_as and 
      mo:Stream, mo:Torrent or mo:ED2K, etc. Therefore, Semantic Web user agents that don't know how to read HTML and even
      less to rip streams from Flash applications can still access the audio content.
  """ ;
  rdfs:domain [ a owl:Class ;
          owl:unionOf ( frbr:Manifestation foaf:Agent mo:CorporateBody ) ] ;
  rdfs:isDefinedBy mo: ;
  rdfs:range foaf:Document ;
  rdfs:subPropertyOf mo:download,
      foaf:isPrimaryTopicOf ;
  vs:term_status "stable" .

mo:listener a owl:ObjectProperty ;
  mo:level "2" ;
  rdfs:comment "Relates a performance to the listener involved" ;
  rdfs:domain mo:Performance ;
  rdfs:isDefinedBy mo: ;
  rdfs:range foaf:Agent ;
  rdfs:subPropertyOf event:agent ;
  owl:inverseOf mo:listened ;
  vs:term_status "stable" .

mo:movement_number a owl:DatatypeProperty ;
  rdfs:label "movement number" ;
  mo:level "2" ;
  rdfs:comment "Indicates the position of a movement in a musical work." ;
  rdfs:domain mo:Movement ;
  rdfs:isDefinedBy mo: ;
  rdfs:range xsd:int ;
  vs:term_status "unstable" .

mo:paid_download a owl:ObjectProperty ;
  rdfs:label "paid download" ;
  mo:level "1" ;
  rdfs:comment """
              Provide a link from an artist to a web page where all of that artist's musical work is available for some money,
              or a link from a manifestation (record/track, for example) to a web page providing a paid access to this manifestation.
      """ ;
  rdfs:domain [ a owl:Class ;
          owl:unionOf ( frbr:Manifestation mo:MusicArtist mo:CorporateBody ) ] ;
  rdfs:isDefinedBy mo: ;
  rdfs:range foaf:Document ;
  rdfs:subPropertyOf mo:download,
      foaf:isPrimaryTopicOf ;
  vs:term_status "stable" .

mo:produced a owl:ObjectProperty ;
  rdfs:label "produced" ;
  mo:level "1" ;
  rdfs:comment "Used to relate an person or a group of person who produced the manifestation of a work." ;
  rdfs:domain foaf:Agent ;
  rdfs:isDefinedBy mo: ;
  rdfs:range mo:MusicalManifestation ;
  owl:inverseOf mo:producer ;
  vs:term_status "stable" .

mo:produced_signal a owl:ObjectProperty ;
  rdfs:label "produced signal" ;
  mo:level "2" ;
  rdfs:comment """
              Associates a Recording to the outputted signal.
      """ ;
  rdfs:domain mo:Recording ;
  rdfs:isDefinedBy mo: ;
  rdfs:range mo:Signal ;
  rdfs:subPropertyOf event:product ;
  vs:term_status "stable" .

mo:produced_sound a owl:ObjectProperty ;
  rdfs:label "produced sound" ;
  mo:level "2" ;
  rdfs:comment """
              Associates a Performance to a physical Sound that is being produced by it.
      """ ;
  rdfs:domain mo:Performance ;
  rdfs:isDefinedBy mo: ;
  rdfs:range mo:Sound ;
  rdfs:subPropertyOf event:product ;
  vs:term_status "stable" .

mo:producer a owl:ObjectProperty ;
  rdfs:label "producer" ;
  mo:level "1" ;
  rdfs:comment "Used to relate the manifestation of a work to a person or a group of person who produced it." ;
  rdfs:domain mo:MusicalManifestation ;
  rdfs:isDefinedBy mo: ;
  rdfs:range foaf:Agent ;
  owl:inverseOf mo:produced ;
  vs:term_status "stable" .

mo:published a owl:ObjectProperty ;
  rdfs:label "published" ;
  mo:level "1" ;
  rdfs:comment "Used to relate an person or a group of person who published the manifestation of a work." ;
  rdfs:domain foaf:Agent ;
  rdfs:isDefinedBy mo: ;
  rdfs:range mo:MusicalManifestation ;
  owl:inverseOf mo:publisher ;
  vs:term_status "unstable" .

mo:publisher a owl:ObjectProperty ;
  rdfs:label "publisher" ;
  mo:level "1" ;
  rdfs:comment "Used to relate a musical manifestation to a person or a group of person who published it." ;
  rdfs:domain mo:MusicalManifestation ;
  rdfs:isDefinedBy mo: ;
  rdfs:range foaf:Agent ;
  owl:inverseOf mo:published ;
  vs:term_status "unstable" .

mo:publishing_location a owl:ObjectProperty ;
  rdfs:label "publishingLocation" ;
  mo:level "1" ;
  rdfs:comment """
      Relates a musical manifestation to its publication location.
      """ ;
  rdfs:domain mo:MusicalManifestation ;
  rdfs:isDefinedBy mo: ;
  rdfs:range geo:SpatialThing ;
  vs:term_status "stable" .

mo:recordedAs a owl:ObjectProperty ;
  owl:equivalentProperty mo:recorded_as .

mo:recorded_as a owl:ObjectProperty ;
  rdfs:label "recorded as" ;
  mo:level "2" ;
  rdfs:comment """
      This is a shortcut property, allowing to bypass all the Sound/Recording steps. This property
      allows to directly link a Performance to the recorded Signal. This is recommended for "normal"
      users. However, advanced users wanting to express things such as the location of the microphone will
      have to create this shortcut as well as the whole workflow, in order to let the "normal" users access
      simply the, well, simple information:-) .
  """ ;
  rdfs:domain mo:Performance ;
  rdfs:isDefinedBy mo: ;
  rdfs:range mo:Signal ;
  owl:inverseOf mo:records ;
  vs:term_status "stable" .

mo:records a owl:ObjectProperty ;
  rdfs:label "records" ;
  mo:level "2" ;
  rdfs:comment """
      This is the inverse of the shortcut property recordedAs, allowing to relate directly a performance
      to a signal.
  """ ;
  rdfs:domain mo:Signal ;
  rdfs:isDefinedBy mo: ;
  rdfs:range mo:Performance ;
  owl:inverseOf mo:recordedAs ;
  vs:term_status "unstable" .

mo:release_status a owl:ObjectProperty ;
  mo:level "1" ;
  rdfs:comment """
              Relates a musical manifestation to its release status (bootleg, ...)
      """ ;
  rdfs:domain mo:MusicalManifestation ;
  rdfs:isDefinedBy mo: ;
  rdfs:range mo:ReleaseStatus ;
  vs:term_status "stable" .

mo:release_type a owl:ObjectProperty ;
  mo:level "1" ;
  rdfs:comment """
      Relates a musical manifestation to its release type (interview, spoken word, album, ...)
  """ ;
  rdfs:domain mo:MusicalManifestation ;
  rdfs:isDefinedBy mo: ;
  rdfs:range mo:ReleaseType ;
  vs:term_status "stable" .

mo:remixed a owl:ObjectProperty ;
  rdfs:label "remixed" ;
  mo:level "1" ;
  rdfs:comment """Used to relate an artist who remixed a musical work or the expression of a musical work. 

This involves taking just one other musical work and using audio editing to make it sound like a significantly different, but usually still recognisable, song. It can be used to link an artist to a single song that they remixed, or, if they remixed an entire musical work.""" ;
  rdfs:domain mo:MusicArtist ;
  rdfs:isDefinedBy mo: ;
  rdfs:range mo:Signal ;
  owl:inverseOf mo:remixer ;
  vs:term_status "unstable" .

mo:remixer a owl:ObjectProperty ;
  rdfs:label "remixer" ;
  mo:level "1" ;
  rdfs:comment """Used to relate a musical work or the expression of a musical work to an artist who remixed it. 

This involves taking just one other musical work and using audio editing to make it sound like a significantly different, but usually still recognisable, song. It can be used to link an artist to a single song that they remixed, or, if they remixed an entire musical work.""" ;
  rdfs:isDefinedBy mo: ;
  rdfs:subPropertyOf mo:interpreter ;
  owl:inverseOf mo:remixed ;
  vs:term_status "unstable" .

mo:sample_rate a owl:DatatypeProperty,
      owl:FunctionalProperty ;
  mo:level "1" ;
  rdfs:comment """
      Associates a digital signal to its sample rate. It might be easier to express it this way instead of
      defining a timeline map:-) Range is xsd:float.
  """ ;
  rdfs:domain mo:DigitalSignal ;
  rdfs:isDefinedBy mo: ;
  rdfs:range xsd:float ;
  vs:term_status "stable" .

mo:sampled a owl:ObjectProperty ;
  rdfs:label "sampled" ;
  mo:level "1" ;
  rdfs:comment "Used to relate an artist who sampled a Signal." ;
  rdfs:domain mo:MusicArtist ;
  rdfs:isDefinedBy mo: ;
  rdfs:range mo:Signal ;
  owl:inverseOf mo:sampler ;
  vs:term_status "unstable" .

mo:sampled_version a owl:ObjectProperty ;
  rdfs:label "sampled version" ;
  mo:level "2" ;
  rdfs:comment """
      Associates an analog signal with a sampled version of it
  """ ;
  rdfs:domain mo:AnalogSignal ;
  rdfs:isDefinedBy mo: ;
  rdfs:range mo:DigitalSignal ;
  owl:inverseOf mo:sampled_version_of ;
  vs:term_status "stable" .

mo:sampler a owl:ObjectProperty ;
  rdfs:label "sampler" ;
  mo:level "1" ;
  rdfs:comment "Used to relate the signal of a musical work to an artist who sampled it." ;
  rdfs:isDefinedBy mo: ;
  rdfs:subPropertyOf mo:interpreter ;
  owl:inverseOf mo:sampled ;
  vs:term_status "unstable" .

mo:time a owl:FunctionalProperty,
      owl:ObjectProperty ;
  rdfs:label "time" ;
  mo:level "1" ;
  rdfs:comment """
      Associates a Signal to a time object - its actual domain
  """ ;
  rdfs:domain mo:Signal ;
  rdfs:isDefinedBy mo: ;
  rdfs:range time:TemporalEntity ;
  vs:term_status "stable" .

mo:track a owl:ObjectProperty ;
  rdfs:label "track" ;
  mo:level "1" ;
  rdfs:comment "Indicates a part of a musical manifestation - in this particular case, a track." ;
  rdfs:domain mo:Record ;
  rdfs:isDefinedBy mo: ;
  rdfs:range mo:Track ;
  vs:term_status "stable" .

mo:track_number a owl:DatatypeProperty ;
  rdfs:label "track number" ;
  mo:level "1" ;
  rdfs:comment "Indicates the position of a track on a record medium (a CD, etc.)." ;
  rdfs:domain mo:Track ;
  rdfs:isDefinedBy mo: ;
  rdfs:range xsd:nonNegativeInteger ;
  vs:term_status "stable" .

mo:Lyrics a owl:Class ;
  rdfs:label "lyrics" ;
  mo:level "2" ;
  rdfs:comment """
      Lyrics
  """ ;
  rdfs:isDefinedBy mo: ;
  rdfs:subClassOf mo:MusicalExpression ;
  vs:term_status "stable" .

mo:Movement a owl:Class ;
  rdfs:label "movement" ;
  mo:level "2" ;
  rdfs:comment """A movement is a self-contained part of a musical work. While individual or selected movements from a composition are sometimes performed separately, a performance of the complete work requires all the movements to be performed in succession.

Often a composer attempts to interrelate the movements thematically, or sometimes in more subtle ways, in order that the individual
movements exert a cumulative effect. In some forms, composers sometimes link the movements, or ask for them to be played without a
pause between them.
  """ ;
  rdfs:isDefinedBy mo: ;
  rdfs:subClassOf mo:MusicalWork ;
  vs:term_status "unstable" .

mo:ReleaseEvent a owl:Class ;
  rdfs:label "release event" ;
  mo:level "1" ;
  rdfs:comment "A release event, in a particular place (e.g. a country) at a particular time. Other factors of this event might include cover art, liner notes, box, etc. or a release grouping all these." ;
  rdfs:isDefinedBy mo: ;
  rdfs:subClassOf event:Event ;
  vs:term_status "testing" .

mo:composed_in a owl:ObjectProperty ;
  rdfs:label "composed in" ;
  mo:level "2" ;
  rdfs:comment """
      Associates a MusicalWork to the Composition event pertaining
      to its creation. For example, I might use this property to associate
      the Magic Flute to its composition event, occuring during 1782 and having as
      a mo:composer Mozart.
  """ ;
  rdfs:domain mo:MusicalWork ;
  rdfs:isDefinedBy mo: ;
  rdfs:range mo:Composition ;
  rdfs:subPropertyOf event:producedIn ;
  owl:inverseOf mo:produced_work ;
  vs:term_status "unstable" .

mo:conducted a owl:ObjectProperty ;
  rdfs:label "conducted" ;
  mo:level "2" ;
  rdfs:comment "Relates agents to the performances they were conducting" ;
  rdfs:domain foaf:Agent ;
  rdfs:isDefinedBy mo: ;
  rdfs:range mo:Performance ;
  rdfs:subPropertyOf event:isAgentIn,
      bio:event ;
  owl:inverseOf mo:conductor ;
  vs:term_status "unstable" .

mo:engineered a owl:ObjectProperty ;
  rdfs:label "engineered" ;
  mo:level "2" ;
  rdfs:comment "Relates agents to the performances/recordings they were engineering in" ;
  rdfs:domain foaf:Agent ;
  rdfs:isDefinedBy mo: ;
  rdfs:range [ a owl:Class ;
          owl:unionOf ( mo:Performance mo:Recording mo:RecordingSession ) ] ;
  rdfs:subPropertyOf event:isAgentIn,
      bio:event ;
  owl:inverseOf mo:engineer ;
  vs:term_status "unstable" .

mo:gtin a owl:DatatypeProperty ;
  rdfs:label "gtin" ;
  mo:level "1" ;
  rdfs:comment "GTIN is a grouping term for EANs and UPCs. In common speech those are called barcodes although the barcodes are just a representation of those identifying numbers." ;
  rdfs:domain mo:Release ;
  rdfs:isDefinedBy mo: ;
  rdfs:range xsd:string ;
  vs:term_status "testing" .

mo:interpreter a owl:ObjectProperty ;
  rdfs:label "has interpeter" ;
  mo:level "1" ;
  rdfs:comment "Adds an involved music artist, who interpreted, remixed, or otherwise modified an existing signal, which resulted in the signal that is here the subject of this relation." ;
  rdfs:domain mo:Signal ;
  rdfs:isDefinedBy mo: ;
  rdfs:range mo:MusicArtist ;
  vs:term_status "testing" .

mo:listened a owl:ObjectProperty ;
  rdfs:label "listened" ;
  mo:level "2" ;
  rdfs:comment "Relates agents to the performances they were listening in" ;
  rdfs:domain foaf:Agent ;
  rdfs:isDefinedBy mo: ;
  rdfs:range mo:Performance ;
  rdfs:subPropertyOf event:isAgentIn,
      bio:event ;
  owl:inverseOf mo:listener ;
  vs:term_status "unstable" .

mo:performance_of a owl:ObjectProperty ;
  rdfs:label "performance of" ;
  mo:level "2" ;
  rdfs:comment """
      Associates a Performance to a musical work or an arrangement that is being used as a factor in it.
      For example, I might use this property to attach the Magic Flute musical work to 
      a particular Performance.
  """ ;
  rdfs:domain mo:Performance ;
  rdfs:isDefinedBy mo: ;
  rdfs:range [ a owl:Class ;
          owl:unionOf ( mo:Score mo:MusicalWork ) ] ;
  rdfs:subPropertyOf event:factor ;
  owl:inverseOf mo:performed_in ;
  vs:term_status "unstable" .

mo:performed a owl:ObjectProperty ;
  rdfs:label "performed" ;
  mo:level "2" ;
  rdfs:comment "Relates agents to the performances they were performing in" ;
  rdfs:domain foaf:Agent ;
  rdfs:isDefinedBy mo: ;
  rdfs:range mo:Performance ;
  rdfs:subPropertyOf event:isAgentIn,
      bio:event ;
  owl:inverseOf mo:performer ;
  vs:term_status "unstable" .

mo:performed_in a owl:ObjectProperty ;
  rdfs:label "performed in" ;
  mo:level "2" ;
  rdfs:comment """
      Associates a Musical Work or an Score to Performances in which they were
      a factor. For example, I might use this property in order to 
      associate the Magic Flute to a particular performance at the Opera
      Bastille last year.""" ;
  rdfs:domain [ a owl:Class ;
          owl:unionOf ( mo:Score mo:MusicalWork ) ] ;
  rdfs:isDefinedBy mo: ;
  rdfs:range mo:Performance ;
  rdfs:subPropertyOf event:isFactorOf ;
  owl:inverseOf mo:performance_of ;
  vs:term_status "unstable" .

mo:produced_work a owl:ObjectProperty ;
  rdfs:label "produced work" ;
  mo:level "2" ;
  rdfs:comment """
              Associates a composition event to the produced MusicalWork. For example,
              this property could link the event corresponding to the composition of the
              Magic Flute in 1782 to the Magic Flute musical work itself. This musical work
              can then be used in particular performances.
      """ ;
  rdfs:domain mo:Composition ;
  rdfs:isDefinedBy mo: ;
  rdfs:range mo:MusicalWork ;
  rdfs:subPropertyOf event:product ;
  owl:inverseOf mo:composed_in ;
  vs:term_status "stable" .

mo:publication_of a owl:ObjectProperty ;
  rdfs:label "publication of" ;
  mo:level "1" ;
  rdfs:comment "Link a particular manifestation to the related signal, score, libretto, or lyrics" ;
  rdfs:domain mo:MusicalManifestation ;
  rdfs:isDefinedBy mo: ;
  rdfs:range mo:MusicalExpression ;
  owl:inverseOf mo:published_as ;
  vs:term_status "unstable" .

mo:published_as a owl:ObjectProperty ;
  rdfs:label "published as" ;
  mo:level "1" ;
  rdfs:comment """
      Links a musical expression (e.g. a signal or a score) to one of its manifestations (e.g. a track on a particular record or a published score).
  """ ;
  rdfs:domain mo:MusicalExpression ;
  rdfs:isDefinedBy mo: ;
  rdfs:range mo:MusicalManifestation ;
  rdfs:subPropertyOf frbr:embodiment ;
  owl:inverseOf mo:publication_of ;
  vs:term_status "stable" .

mo:recorded_in a owl:ObjectProperty ;
  rdfs:label "recorded in" ;
  mo:level "2" ;
  rdfs:comment """
          Associates a physical Sound to a Recording event where it is being used 
      in order to produce a signal. For example, I might use this property to 
      associate the sound produced by a particular performance of the magic flute
      to a given recording, done using my cell-phone.
  """ ;
  rdfs:domain mo:Sound ;
  rdfs:isDefinedBy mo: ;
  rdfs:range mo:Recording ;
  rdfs:subPropertyOf event:isFactorOf ;
  owl:inverseOf mo:recording_of ;
  vs:term_status "unstable" .

mo:recording_of a owl:ObjectProperty ;
  rdfs:label "recorded sound" ;
  mo:level "2" ;
  rdfs:comment """
          Associates a Recording event to a physical Sound being recorded.
              For example, I might use this property to
              associate a given recording, done using my cell phone, to the 
      sound produced by a particular performance of the magic flute.
  """ ;
  rdfs:domain mo:Recording ;
  rdfs:isDefinedBy mo: ;
  rdfs:range mo:Sound ;
  rdfs:subPropertyOf event:factor ;
  owl:inverseOf mo:recorded_in ;
  vs:term_status "stable" .

mo:sampled_version_of a owl:FunctionalProperty,
      owl:ObjectProperty ;
  rdfs:label "sampled version of" ;
  mo:level "2" ;
  rdfs:comment """
      Associates a digital signal with the analog version of it
  """ ;
  rdfs:domain mo:DigitalSignal ;
  rdfs:isDefinedBy mo: ;
  rdfs:range mo:AnalogSignal ;
  rdfs:subPropertyOf mo:derived_from ;
  owl:inverseOf mo:sampled_version ;
  vs:term_status "stable" .

mo:AnalogSignal a owl:Class ;
  rdfs:label "analogue signal" ;
  mo:level "2" ;
  rdfs:comment """
      An analog signal.
  """ ;
  rdfs:isDefinedBy mo: ;
  rdfs:subClassOf mo:Signal ;
  owl:disjointWith mo:DigitalSignal ;
  vs:term_status "stable" .

mo:Instrument a owl:Class ;
  rdfs:label "Instrument" ;
  mo:level "2" ;
  rdfs:comment """
      Any of various devices or contrivances that can be used to produce musical tones or sound.

      Any taxonomy can be used to subsume this concept. The default one is one extracted by Ivan Herman
      from the Musicbrainz instrument taxonomy, conforming to SKOS. This concept holds a seeAlso link 
      towards this taxonomy.
  """ ;
  rdfs:isDefinedBy mo: ;
  rdfs:seeAlso <http://purl.org/ontology/mo/mit#> ;
  vs:term_status "stable" .

mo:Label a owl:Class ;
  rdfs:label "label" ;
  mo:level "1" ;
  rdfs:comment "Trade name of a company that produces musical works or expression of musical works." ;
  rdfs:isDefinedBy mo: ;
  rdfs:subClassOf mo:CorporateBody ;
  vs:term_status "stable" .

mo:SignalGroup a owl:Class ;
  rdfs:label "signal group" ;
  mo:level "1" ;
  rdfs:comment """
      A musical expression representing a group of signals, for example a set of masters resulting from a whole recording/mastering session.
  """ ;
  rdfs:isDefinedBy mo: ;
  rdfs:subClassOf mo:MusicalExpression ;
  vs:term_status "testing" .

mo:Sound a owl:Class ;
  rdfs:label "sound" ;
  mo:level "2" ;
  rdfs:comment """
      A subclass of MusicalExpression, representing a sound. Realisation of a MusicalWork during a musical Performance.
  """ ;
  rdfs:isDefinedBy mo: ;
  rdfs:subClassOf event:Event,
      mo:MusicalExpression ;
  vs:term_status "stable" .

mo:available_as a owl:ObjectProperty ;
  mo:level "1" ;
  rdfs:comment """
      Relates a musical manifestation to a musical item (this album, and my particular cd). By using
      this property, there is no assumption on wether the full content is available on the linked item.
      To be explicit about this, you can use a sub-property, such as mo:item (the full manifestation
      is available on that item) or mo:preview (only a part of the manifestation is available on
      that item).

      This is a subproperty of frbr:examplar.
  """ ;
  rdfs:domain mo:MusicalManifestation ;
  rdfs:isDefinedBy mo: ;
  rdfs:range mo:MusicalItem ;
  rdfs:subPropertyOf frbr:exemplar ;
  vs:term_status "stable" .

mo:download a owl:ObjectProperty ;
  rdfs:label "download" ;
  mo:level "1" ;
  rdfs:comment """
              This property can be used to link from a person to the website where they make their works available, or from
              a manifestation (a track or an album, for example) to a web page where it is available for
              download.

      It is better to use one of the three sub-properties instead of this one in order to specify wether the
      content can be accessed for free (mo:freedownload), if it is just free preview material (mo:previewdownload), or
      if it can be accessed for some money (mo:paiddownload) (this includes links to the Amazon store, for example).

              This property MUST be used only if the content is just available through a web page (holding, for example
              a Flash application) - it is better to link to actual content directly through the use of mo:available_as and
              mo:Stream, mo:Torrent or mo:ED2K, etc. Therefore, Semantic Web user agents that don't know how to read HTML and even
              less to rip streams from Flash applications can still access the audio content.
      """ ;
  rdfs:domain [ a owl:Class ;
          owl:unionOf ( frbr:Manifestation foaf:Agent mo:CorporateBody ) ] ;
  rdfs:isDefinedBy mo: ;
  rdfs:range foaf:Document ;
  rdfs:subPropertyOf foaf:isPrimaryTopicOf ;
  vs:term_status "stable" .

mo:performer a owl:ObjectProperty ;
  mo:level "2" ;
  rdfs:comment "Relates a performance to the performers involved" ;
  rdfs:domain mo:Performance ;
  rdfs:isDefinedBy mo: ;
  rdfs:range foaf:Agent ;
  rdfs:subPropertyOf event:agent ;
  owl:inverseOf mo:performed ;
  vs:term_status "stable" .

mo:Genre a owl:Class ;
  rdfs:label "Genre" ;
  mo:level "2" ;
  rdfs:comment """
      An expressive style of music.

      Any taxonomy can be plug-in here. You can either define a genre by yourself, like this:

      :mygenre a mo:Genre; dc:title "electro rock".

      Or you can refer to a DBPedia genre (such as http://dbpedia.org/resource/Baroque_music), allowing semantic web
      clients to access easily really detailed structured information about the genre you are refering to.
  """ ;
  rdfs:isDefinedBy mo: ;
  vs:term_status "stable" .

mo:Membership a owl:Class ;
  rdfs:label "membership" ;
  mo:level "1" ;
  rdfs:comment "A membership event, where one or several people belongs to a group during a particular time period." ;
  rdfs:isDefinedBy mo: ;
  rdfs:subClassOf event:Event ;
  vs:term_status "testing" .

mo:RecordingSession a owl:Class ;
  rdfs:label "recording session" ;
  mo:level "2" ;
  rdfs:comment "A set of performances/recordings/mastering events. This event can be decomposed in its constituent events using event:sub_event" ;
  rdfs:isDefinedBy mo: ;
  rdfs:subClassOf event:Event ;
  vs:term_status "testing" .

mo:ReleaseStatus a owl:Class ;
  rdfs:label "release status" ;
  mo:level "1" ;
  rdfs:comment "Musical manifestation release status." ;
  rdfs:isDefinedBy mo: ;
  vs:term_status "stable" .

mo:Score a owl:Class ;
  rdfs:label "score" ;
  mo:level "2" ;
  rdfs:comment """
      Here, we are dealing with the informational object (the MusicalExpression), not the actually "published" score.
      This may be, for example, the product of an arrangement process.
  """ ;
  rdfs:isDefinedBy mo: ;
  rdfs:subClassOf mo:MusicalExpression ;
  vs:term_status "stable" .

mo:Composition a owl:Class ;
  rdfs:label "composition" ;
  mo:level "2" ;
  rdfs:comment """
      A composition event.
      Takes as agent the composer himself.
      It produces a MusicalWork, or a MusicalExpression (when the initial "product" is a score, for example), or both...
  """ ;
  rdfs:isDefinedBy mo: ;
  rdfs:subClassOf event:Event ;
  vs:term_status "stable" .

mo:DigitalSignal a owl:Class ;
  rdfs:label "digital signal" ;
  mo:level "2" ;
  rdfs:comment """
      A digital signal
  """ ;
  rdfs:isDefinedBy mo: ;
  rdfs:subClassOf mo:Signal ;
  owl:disjointWith mo:AnalogSignal ;
  vs:term_status "stable" .

mo:Record a owl:Class ;
  rdfs:label "record" ;
  mo:level "1" ;
  rdfs:comment "A published record (manifestation which first aim is to render the product of a recording)" ;
  rdfs:isDefinedBy mo: ;
  rdfs:subClassOf mo:MusicalManifestation ;
  vs:term_status "stable" .

mo:Recording a owl:Class ;
  rdfs:label "recording" ;
  mo:level "2" ;
  rdfs:comment """
      A recording event.
      Takes a sound as a factor to produce a signal (analog or digital).
      The location of such events (if any) is the actual location of the corresponding
      microphone or the "recording device".
  """ ;
  rdfs:isDefinedBy mo: ;
  rdfs:subClassOf event:Event ;
  vs:term_status "stable" .

mo:Track a owl:Class ;
  rdfs:label "rack" ;
  mo:level "1" ;
  rdfs:comment "A track on a particular record" ;
  rdfs:isDefinedBy mo: ;
  rdfs:subClassOf mo:MusicalManifestation ;
  vs:term_status "stable" .

mo:Arrangement a owl:Class ;
  rdfs:label "arrangement" ;
  mo:level "2" ;
  rdfs:comment """
      An arrangement event.
      Takes as agent the arranger, and produces a score (informational object, not the actually published score).
  """ ;
  rdfs:isDefinedBy mo: ;
  rdfs:subClassOf event:Event ;
  vs:term_status "stable" .

mo:derived_from a owl:ObjectProperty ;
  rdfs:label "derived from" ;
  mo:level "1" ;
  rdfs:comment "A related signal from which the described signal is derived." ;
  rdfs:domain mo:Signal ;
  rdfs:isDefinedBy mo: ;
  rdfs:range mo:Signal ;
  rdfs:subPropertyOf dcterms:source ;
  vs:term_status "testing" .

mo:CorporateBody a owl:Class ;
  rdfs:label "corporate body" ;
  mo:level "1" ;
  rdfs:comment "Organization or group of individuals and/or other organizations involved in the music market." ;
  rdfs:isDefinedBy mo: ;
  rdfs:subClassOf foaf:Organization ;
  vs:term_status "stable" .

mo:uuid a owl:DatatypeProperty ;
  rdfs:label "universally unique identifier" ;
  mo:level "1" ;
  rdfs:comment """
          Links an object to an universally unique identifier for it.
  """ ;
  rdfs:domain owl:Thing ;
  rdfs:subPropertyOf dcterms:identifier ;
  vs:term_status "testing" .

mo:Release a owl:Class ;
  rdfs:label "release" ;
  mo:level "1" ;
  rdfs:comment "A specific release, with barcode, box, liner notes, cover art, and a number of records" ;
  rdfs:isDefinedBy mo: ;
  rdfs:subClassOf mo:MusicalManifestation ;
  vs:term_status "testing" .

mo:MusicalItem a owl:Class ;
  rdfs:label "MusicalItem" ;
  mo:level "1" ;
  rdfs:comment """A single exemplar of a musical expression.

For example, it could be a single exemplar of a CD. This is normally an single object (a CD) possessed by somebody.

From the FRBR final report: The entity defined as item is a concrete entity. It is in many instances a single physical object (e.g., a copy of a one-volume monograph, a single audio cassette, etc.). There are instances, however, where the entity defined as item comprises more than one physical object (e.g., a monograph issued as two separately bound volumes, a recording issued on three separate compact discs, etc.).

In terms of intellectual content and physical form, an item exemplifying a manifestation is normally the same as the manifestation itself. However, variations may occur from one item to another, even when the items exemplify the same manifestation, where those variations are the result of actions external to the intent of the producer of the manifestation (e.g., damage occurring after the item was produced, binding performed by a library, etc.). 
  """ ;
  rdfs:isDefinedBy mo: ;
  vs:term_status "unstable" .

mo:ReleaseType a owl:Class ;
  rdfs:label "Release type" ;
  mo:level "1" ;
  rdfs:comment """
      Release type of a particular manifestation, such as "album" or "interview"...
  """ ;
  rdfs:isDefinedBy mo: ;
  vs:term_status "stable" .

mo:Medium a owl:Class ;
  rdfs:label "Medium" ;
  mo:level "1" ;
  rdfs:comment "A means or instrumentality for storing or communicating musical manifestation." ;
  rdfs:isDefinedBy mo: ;
  rdfs:subClassOf mo:MusicalItem ;
  vs:term_status "unstable" .

mo:MusicalExpression a owl:Class ;
  rdfs:label "musical expression" ;
  mo:level "1" ;
  rdfs:comment """
The intellectual or artistic realization of a work in the form of alpha-numeric, musical, or choreographic notation, sound, etc., or any combination of such forms.    


For example:

Work #1 Franz Schubert's Trout quintet

  * Expression #1 the composer's score
  * Expression #2 sound issued from the performance by the Amadeus Quartet and Hephzibah Menuhin on piano
  * Expression #3 sound issued from the performance by the Cleveland Quartet and Yo-Yo Ma on the cello
  * . . . . 

The Music Ontology defines the following sub-concepts of a MusicalExpression, which should be used instead of MusicalExpression itself: Score (the
result of an arrangement), Sound (produced during a performance), Signal. However, it is possible to stick to FRBR and bypass the worflow
mechanism this ontology defines by using the core FRBR properties on such objects. But it is often better to use events to interconnect such 
expressions (allowing to go deeply into the production process - `this performer was playing this particular instrument at that
particular time').

  """ ;
  rdfs:isDefinedBy mo: ;
  rdfs:subClassOf frbr:Expression ;
  vs:term_status "unstable" .

mo:Performance a owl:Class ;
  rdfs:label "performance" ;
  mo:level "2" ;
  rdfs:comment """
      A performance event. 
      It might include as agents performers, engineers, conductors, or even listeners.
      It might include as factors a score, a MusicalWork, musical instruments. 
      It might produce a sound:-)
  """ ;
  rdfs:isDefinedBy mo: ;
  rdfs:subClassOf event:Event ;
  vs:term_status "stable" .

mo:MusicalWork a owl:Class ;
  rdfs:label "musical work" ;
  mo:level "2" ;
  rdfs:comment """
  Distinct intellectual or artistic musical creation.

From the FRBR final report: A work is an abstract entity; there is no single material object one can point to as the work. We recognize the work through individual realizations or expressions of the work, but the work itself exists only in the commonality of
content between and among the various expressions of the work. When we speak of Homer's Iliad as a work, our point of reference is not a particular recitation or text of the work, but the intellectual creation that lies behind all the various expressions of the work.     

For example:

work #1 J. S. Bach's The art of the fugue


  """ ;
  rdfs:isDefinedBy mo: ;
  rdfs:subClassOf frbr:Work ;
  vs:term_status "stable" .

mo:Signal a owl:Class ;
  rdfs:label "signal" ;
  mo:level "1" ;
  rdfs:comment """
      A subclass of MusicalExpression, representing a signal, for example a master signal produced by a performance and a recording.
  """ ;
  rdfs:isDefinedBy mo: ;
  rdfs:subClassOf mo:MusicalExpression ;
  vs:term_status "stable" .

mo:MusicArtist a owl:Class ;
  rdfs:label "music artist" ;
  mo:level "1" ;
  rdfs:comment """
      A person or a group of people (or a computer :-) ), whose musical 
      creative work shows sensitivity and imagination 
  """ ;
  rdfs:isDefinedBy mo: ;
  rdfs:subClassOf foaf:Agent ;
  vs:term_status "stable" .

mo:MusicalManifestation a owl:Class ;
  rdfs:label "musical manifestation" ;
  mo:level "1" ;
  rdfs:comment """

This entity is related to the edition/production/publication of a musical expression (musical manifestation are closely related with the music industry (their terms, concepts, definitions, methods (production, publication, etc.), etc.)

From the FRBR final report: The entity defined as manifestation encompasses a wide range of materials, including manuscripts, books, periodicals, maps, posters, sound recordings, films, video recordings, CD-ROMs, multimedia kits, etc. As an entity, manifestation represents all the physical objects that bear the same characteristics, in respect to both intellectual content and physical form.


Work #1 J. S. Bach's Six suites for unaccompanied cello

  * Expression #1 sound issued during the performance by Janos Starker recorded in 1963 and 1965
        o Manifestation #1 recordings released on 33 1/3 rpm sound discs in 1965 by Mercury
        o Manifestation #2 recordings re-released on compact disc in 1991 by Mercury 
  * Expression #2 sound issued during the performances by Yo-Yo Ma recorded in 1983
        o Manifestation #1 recordings released on 33 1/3 rpm sound discs in 1983 by CBS Records
        o Manifestation #2 recordings re-released on compact disc in 1992 by CBS Records 

  
Changes that occur deliberately or even inadvertently in the production process that affect the copies result, strictly speaking, in a new manifestation. A manifestation resulting from such a change may be identified as a particular "state" or "issue" of the publication.

Changes that occur to an individual copy after the production process is complete (e.g., the loss of a page, rebinding, etc.) are not considered to result in a new manifestation. That copy is simply considered to be an exemplar (or item) of the manifestation that deviates from the copy as produced.

With the entity defined as manifestation we can describe the physical characteristics of a set of items and the characteristics associated with the production and distribution of that set of items that may be important factors in enabling users to choose a manifestation appropriate to their physical needs and constraints, and to identify and acquire a copy of that manifestation.

Defining manifestation as an entity also enables us to draw relationships between specific manifestations of a work. We can use the relationships between manifestations to identify, for example, the specific publication that was used to create a microreproduction.          

""" ;
  rdfs:isDefinedBy mo: ;
  rdfs:subClassOf frbr:Manifestation ;
  vs:term_status "stable" .

mo: a owl:Ontology ;
  dc:date "$Date: 2010/11/28 17:08:19 $" ;
  dc:description """
      The Music Ontology Specification provides main concepts and 
      properties fo describing music (i.e. artists, albums and tracks) 
      on the Semantic Web. This document contains a RDF description 
      of the Music Ontology.
  """ ;
  dc:title "The Music Ontology" ;
  owl:imports <http://purl.org/NET/c4dm/event.owl>,
      <http://purl.org/NET/c4dm/keys.owl>,
      dcterms:,
      <http://purl.org/ontology/ao/core>,
      bio:,
      <http://purl.org/vocab/frbr/core>,
      <http://www.w3.org/2006/time>,
      foaf: ;
  owl:versionInfo "Revision: 2.1.5" ;
  foaf:maker <http://foaf.me/zazi#me>,
      <http://moustaki.org/foaf.rdf#moustaki>,
      <http://www.talkdigger.com/foaf/fgiasson> .




